@prefix : <http://fdri.ceh.ac.uk/vocab/metadata/> .
@prefix dct: <http://purl.org/dc/terms/> .
@prefix geo: <http://www.w3.org/2003/01/geo/wgs84_pos#> .
@prefix iop: <https://w3id.org/iadopt/ont/> .
@prefix owl: <http://www.w3.org/2002/07/owl#> .
@prefix rdf: <http://www.w3.org/1999/02/22-rdf-syntax-ns#> .
@prefix ssn: <http://www.w3.org/ns/ssn/> .
@prefix xml: <http://www.w3.org/XML/1998/namespace> .
@prefix xsd: <http://www.w3.org/2001/XMLSchema#> .
@prefix dcat: <http://www.w3.org/ns/dcat#> .
@prefix geos: <http://www.opengis.net/ont/geosparql#> .
@prefix prov: <http://www.w3.org/ns/prov#> .
@prefix rdfs: <http://www.w3.org/2000/01/rdf-schema#> .
@prefix skos: <http://www.w3.org/2004/02/skos/core#> .
@prefix sosa: <http://www.w3.org/ns/sosa/> .
@prefix schema: <http://schema.org/> .
@prefix spatialrelations: <http://data.ordnancesurvey.co.uk/ontology/spatialrelations/> .
@base <http://fdri.ceh.ac.uk/vocab/metadata/> .

<http://fdri.ceh.ac.uk/vocab/metadata> rdf:type owl:Ontology ;
                                        owl:imports spatialrelations: ,
                                                    <http://www.opengis.net/ont/geosparql/1.1> ,
                                                    <http://www.w3.org/2006/time#2016> ,
                                                    <http://www.w3.org/ns/dcat3> ,
                                                    ssn:ext ,
                                                    <https://w3id.org/iadopt/ont/1.0.3> ;
                                        rdfs:comment "An ontology for the recording of dataset metadata, provenance information and related reference data for use in the fine-grained metadata store element of the FDRI project."@en ;
                                        rdfs:label "FDRI Fine-grained Metadata Store Ontology"@en ;
                                        owl:versionInfo "0.4.1 DRAFT" .

#################################################################
#    Annotation properties
#################################################################

###  http://www.w3.org/2003/01/geo/wgs84_pos#alt
geo:alt rdf:type owl:AnnotationProperty ;
        rdfs:comment """The WGS84 altitude of a SpatialThing (decimal meters 
above the local reference ellipsoid).""" ;
        rdfs:label "altitude" ;
        rdfs:domain geo:SpatialThing .


###  http://www.w3.org/2003/01/geo/wgs84_pos#location
geo:location rdf:type owl:AnnotationProperty ;
             rdfs:subPropertyOf <http://xmlns.com/foaf/0.1/based_near> ;
             rdfs:range geo:SpatialThing .


###  http://xmlns.com/foaf/0.1/based_near
<http://xmlns.com/foaf/0.1/based_near> rdf:type owl:AnnotationProperty .


#################################################################
#    Object Properties
#################################################################

###  http://fdri.ceh.ac.uk/vocab/metadata/affectedFacility
:affectedFacility rdf:type owl:ObjectProperty ;
                  rdfs:subPropertyOf owl:topObjectProperty ;
                  rdfs:domain :Fault ;
                  rdfs:range :EnvironmentalMonitoringFacility ;
                  rdfs:comment "Relates an `fdri:Fault` to the `fdri:EnvironmentalMonitoringFacility` whose operation is or may be affected by the Fault"@en ;
                  rdfs:label "affected facility"@en .


###  http://fdri.ceh.ac.uk/vocab/metadata/affectedVariable
:affectedVariable rdf:type owl:ObjectProperty ;
                  rdfs:subPropertyOf owl:topObjectProperty ;
                  rdfs:domain :Fault ;
                  rdfs:range :Variable ;
                  rdfs:comment "Relates an `fdri:Fault` to the `fdri:Variable` the observation of which is or may be affected by the fault."@en ;
                  rdfs:label "affected variable"@en .


###  http://fdri.ceh.ac.uk/vocab/metadata/aggregation
:aggregation rdf:type owl:ObjectProperty ;
             rdfs:range :Aggregation ;
             rdfs:comment "Defines the statistical aggregation applied to observations to produce a measure."@en ;
             rdfs:label "aggregation"@en .


###  http://fdri.ceh.ac.uk/vocab/metadata/annotationPropertyScheme
:annotationPropertyScheme rdf:type owl:ObjectProperty ;
                          rdfs:subPropertyOf dcat:themeTaxonomy ;
                          rdfs:range :VariableScheme ;
                          rdfs:comment "References a controlled list of annotation properties used by this catalog."@en ;
                          rdfs:label "annotation property scheme"@en .


###  http://fdri.ceh.ac.uk/vocab/metadata/appliesToFacility
:appliesToFacility rdf:type owl:ObjectProperty ;
                   rdfs:subPropertyOf owl:topObjectProperty ;
                   rdfs:range :EnvironmentalMonitoringFacility ;
                   rdfs:comment "Defines the Environmental Monitoring Facility that a data processing configuration applies to."@en ;
                   rdfs:label "applies to facility"@en .


###  http://fdri.ceh.ac.uk/vocab/metadata/appliesToTimeSeries
:appliesToTimeSeries rdf:type owl:ObjectProperty ;
                     rdfs:range [ rdf:type owl:Class ;
                                  owl:unionOf ( :TimeSeriesDataset
                                                :TimeSeriesDefinition
                                              )
                                ] ;
                     rdfs:comment "Defines the Time-Series Dataset or Time-Series Definition that a Data Processing Configuration is used for."@en ;
                     rdfs:label "applies to time-series"@en .


###  http://fdri.ceh.ac.uk/vocab/metadata/appliesToVariable
:appliesToVariable rdf:type owl:ObjectProperty ;
                   rdfs:subPropertyOf owl:topObjectProperty ;
                   rdfs:range :Variable ;
                   rdfs:comment "Defines the Variable that a Data Processing Configuration is applied to."@en ;
                   rdfs:label "applies to variable"@en .


###  http://fdri.ceh.ac.uk/vocab/metadata/argument
:argument rdf:type owl:ObjectProperty ;
          rdfs:subPropertyOf owl:topObjectProperty ;
          rdfs:range :ConfigurationArgument ;
          rdfs:comment "An argument passed to the Data Processing Method of an Internal Data Processing Configuration."@en ;
          rdfs:label "argument"@en .


###  http://fdri.ceh.ac.uk/vocab/metadata/catchmentScheme
:catchmentScheme rdf:type owl:ObjectProperty ;
                 rdfs:subPropertyOf dcat:themeTaxonomy ;
                 rdfs:range :CatchmentScheme ;
                 rdfs:comment "References a controlled list of Catchment areas referenced by the catalog."@en ;
                 rdfs:label "catchment scheme"@en .


###  http://fdri.ceh.ac.uk/vocab/metadata/certification
:certification rdf:type owl:ObjectProperty ;
               rdfs:comment "A link to the document that certifies the system"@en ;
               rdfs:label "certification"@en .


###  http://fdri.ceh.ac.uk/vocab/metadata/configuration
:configuration rdf:type owl:ObjectProperty ;
               rdfs:range [ rdf:type owl:Class ;
                            owl:unionOf ( :ConfigurationValueSeries
                                          :DataProcessingConfiguration
                                        )
                          ] ;
               rdfs:comment "The current and historical configuration of one or more aspects of the parent resource."@en ;
               rdfs:label "configuration"@en .


###  http://fdri.ceh.ac.uk/vocab/metadata/configurationPropertyScheme
:configurationPropertyScheme rdf:type owl:ObjectProperty ;
                             rdfs:subPropertyOf dcat:themeTaxonomy ;
                             rdfs:range :ConfigurationPropertyScheme ;
                             rdfs:comment "References a controlled list of configuration properties referenced by the catalog."@en ;
                             rdfs:label "configiuration property scheme"@en .


###  http://fdri.ceh.ac.uk/vocab/metadata/contains
:contains rdf:type owl:ObjectProperty .


###  http://fdri.ceh.ac.uk/vocab/metadata/environmentalDomain
:environmentalDomain rdf:type owl:ObjectProperty ;
                     rdfs:range :EnvironmentalDomain ;
                     rdfs:comment "The domain(s) of environmental study that the observations of this facility relate to."@en ;
                     rdfs:label "environmental domain"@en .


###  http://fdri.ceh.ac.uk/vocab/metadata/group
:group rdf:type owl:ObjectProperty ;
       rdfs:range :FacilityGroup ;
       rdfs:comment "Defines the Environmental Monitoring Facility Group that participates in an Environmental Monitoring Facility Group Membership relation."@en ;
       rdfs:label "group"@en .


###  http://fdri.ceh.ac.uk/vocab/metadata/hadConfigurationItem
:hadConfigurationItem rdf:type owl:ObjectProperty ;
                      rdfs:subPropertyOf owl:topObjectProperty ;
                      rdfs:range :ConfigurationItem ;
                      rdfs:comment "The configuration item that was part of the parent configuration at some past period in time."@en ;
                      rdfs:label "had configuration item"@en .


###  http://fdri.ceh.ac.uk/vocab/metadata/hadValue
:hadValue rdf:type owl:ObjectProperty ;
          rdfs:range :TimeBoundPropertyValue ;
          rdfs:comment "Defines a value which a property had at during some past period of time."@en ;
          rdfs:label "had value"@en .


###  http://fdri.ceh.ac.uk/vocab/metadata/hasAnnotation
:hasAnnotation rdf:type owl:ObjectProperty ;
               rdfs:range :Annotation ;
               rdfs:comment "Relates an item to the `fdri:Annotation` items that provide additional property values for that item."@en ;
               rdfs:label "has annotation"@en .


###  http://fdri.ceh.ac.uk/vocab/metadata/hasCurrentConfigurationItem
:hasCurrentConfigurationItem rdf:type owl:ObjectProperty ;
                             rdfs:subPropertyOf owl:topObjectProperty ;
                             rdfs:range :ConfigurationItem ;
                             rdfs:comment "The configuration item that is part of the parent configuration at the present time."@en ;
                             rdfs:label "has current configuration item"@en .


###  http://fdri.ceh.ac.uk/vocab/metadata/hasCurrentValue
:hasCurrentValue rdf:type owl:ObjectProperty ;
                 rdfs:range :TimeBoundPropertyValue ;
                 rdfs:comment "The value that a property currently has."@en ;
                 rdfs:label "has current value"@en .


###  http://fdri.ceh.ac.uk/vocab/metadata/hasMember
:hasMember rdf:type owl:ObjectProperty ;
           rdfs:comment "Represents a simple group-membership relationship in which the subject of the statement is the group and the object of the statement the group member"@en ;
           rdfs:label "has member"@en .


###  http://fdri.ceh.ac.uk/vocab/metadata/hasProcedure
:hasProcedure rdf:type owl:ObjectProperty ;
              rdfs:range :Procedure ;
              rdfs:comment "Relates a resource to a Procedure which may be applied to that resource."@en ;
              rdfs:label "has procedure"@en .


###  http://fdri.ceh.ac.uk/vocab/metadata/hasRepresentativePoint
:hasRepresentativePoint rdf:type owl:ObjectProperty ;
                        rdfs:subPropertyOf geos:hasGeometry ;
                        rdfs:comment "Provides a represenataive point location for an item which may have more complex spatial geometry assocaited with it."@en ;
                        rdfs:label "has representative point"@en .


###  http://fdri.ceh.ac.uk/vocab/metadata/hasUnit
:hasUnit rdf:type owl:ObjectProperty ;
         rdfs:domain :Measure ;
         rdfs:range <http://qudt.org/schema/qudt/Unit> ;
         rdfs:comment "Relates a Measure to the unit of measurement used by observations of the property."@en ;
         rdfs:label "has unit"@en .


###  http://fdri.ceh.ac.uk/vocab/metadata/hasValue
:hasValue rdf:type owl:ObjectProperty ;
          rdfs:subPropertyOf owl:topObjectProperty ;
          rdfs:range schema:PropertyValue ;
          rdfs:comment """Provides the current value of the item (an `fdri:Annotation` or `fdri:ConfigurationValue`).

This property should be used for annotations where it is not necessary to track an historical record of the annotation values over time, and should be used to provide the currently accepted value of the parent item.

When `fdri:hasValueSeries` is present on an item, this property SHOULD NOT be present on the same item."""@en ;
          rdfs:label "has value"@en .


###  http://fdri.ceh.ac.uk/vocab/metadata/hasValueSeries
:hasValueSeries rdf:type owl:ObjectProperty ;
                rdfs:subPropertyOf owl:topObjectProperty ;
                rdfs:range :PropertyValueSeries ;
                rdfs:comment """Provides a historical record of the values of the parent item (an fdri:Annotation) including the current annotation value.

When `fdri:hasValue` is present on an item, this property SHOULD NOT be present on the same item."""@en ;
                rdfs:label "has value series"@en .


###  http://fdri.ceh.ac.uk/vocab/metadata/interval
:interval rdf:type owl:ObjectProperty ;
          rdfs:range dct:PeriodOfTime ;
          rdfs:comment "Relates a time-bound property or relationship to the period of time during which that property or relationship was valid."@en ;
          rdfs:label "interval"@en .


###  http://fdri.ceh.ac.uk/vocab/metadata/measure
:measure rdf:type owl:ObjectProperty ;
         rdfs:domain :ObservationDataset ;
         rdfs:range :Measure ;
         rdfs:comment "Relates an ObservationDataset to a Measure that the dataset provides values for."@en ;
         rdfs:label "measure"@en .


###  http://fdri.ceh.ac.uk/vocab/metadata/measures
:measures rdf:type owl:ObjectProperty ;
          rdfs:range :Measure ;
          rdfs:comment "Relates a resource to the `fdri:Measure` that the resource has capacity to measure."@en ;
          rdfs:label "measures"@en .


###  http://fdri.ceh.ac.uk/vocab/metadata/member
:member rdf:type owl:ObjectProperty ;
        rdfs:range :EnvironmentalMonitoringFacility ;
        rdfs:comment "Defines the Environmental Monitoring Facility that is a member of some Environmental Monitoring Facility Group in a qualified Environmental Monitoring Facility Group Membership relationship."@en ;
        rdfs:label "member"@en .


###  http://fdri.ceh.ac.uk/vocab/metadata/method
:method rdf:type owl:ObjectProperty ;
        rdfs:subPropertyOf owl:topObjectProperty ;
        rdfs:domain skos:Concept ;
        rdfs:comment "Relates a Data Processing Configuration Item to the data processing method that is configured."@en ;
        rdfs:label "method"@en .


###  http://fdri.ceh.ac.uk/vocab/metadata/methodology
:methodology rdf:type owl:ObjectProperty ;
             rdfs:range prov:Plan ;
             rdfs:comment "Relates a Time-Series Definition to the Plan that defines how instances of the Time-Series Definition are generated and/or updated."@en ;
             rdfs:label "methodology"@en .


###  http://fdri.ceh.ac.uk/vocab/metadata/monitoringFacilityTypeScheme
:monitoringFacilityTypeScheme rdf:type owl:ObjectProperty ;
                              rdfs:subPropertyOf dcat:themeTaxonomy ;
                              rdfs:range :EnvironmentalMonitoringFacilityTypeScheme ;
                              rdfs:comment "References a controlled list of monintoring facility types referenced by the catalog."@en ;
                              rdfs:label "monitoring facility type scheme"@en .


###  http://fdri.ceh.ac.uk/vocab/metadata/monitoringSystemTypeScheme
:monitoringSystemTypeScheme rdf:type owl:ObjectProperty ;
                            rdfs:subPropertyOf dcat:themeTaxonomy ;
                            rdfs:range :EnvironmentalMonitoringFacilityTypeScheme ;
                            rdfs:comment "References a controlled list of monitoring system types referenced by the catalog."@en ;
                            rdfs:label "monitoring system type scheme"@en .


###  http://fdri.ceh.ac.uk/vocab/metadata/observationInterval
:observationInterval rdf:type owl:ObjectProperty ;
                     rdfs:subPropertyOf owl:topObjectProperty ;
                     rdfs:range dct:PeriodOfTime ;
                     rdfs:comment "Defines a time-slice of observations that a configuration item applies to. This is distinct from the `interval` which defines the period during which the configuration item is/was used in data processing."@en ;
                     rdfs:label "observation interval"@en .


###  http://fdri.ceh.ac.uk/vocab/metadata/observedPropertyScheme
:observedPropertyScheme rdf:type owl:ObjectProperty ;
                        rdfs:subPropertyOf dcat:themeTaxonomy ;
                        rdfs:range :VariableScheme ;
                        rdfs:comment "References a controlled vocabulary of Variables that is referenced by the catalog."@en ;
                        rdfs:label "observed property scheme"@en .


###  http://fdri.ceh.ac.uk/vocab/metadata/operatingPeriod
:operatingPeriod rdf:type owl:ObjectProperty ;
                 rdfs:range dct:PeriodOfTime ;
                 rdfs:comment "The period of time during which an Environmental Monitoring Facility is/was operational."@en ;
                 rdfs:label "operating period"@en .


###  http://fdri.ceh.ac.uk/vocab/metadata/originatingFacility
:originatingFacility rdf:type owl:ObjectProperty ;
                     rdfs:subPropertyOf owl:topObjectProperty ;
                     rdfs:domain :ObservationDataset ;
                     rdfs:range :EnvironmentalMonitoringFacility ;
                     rdfs:comment "Relates a dataset of observations to the Environmental Monitoring Facility from which the observations originated. The choice of facilit(ies) to use as the value of this property should be restricted to those which apply to all observations in the temporal range of the dataset (such as a site or a platform), and not to facilities which might be replaced over the time span of the dataset (such as a replacable sensor or sensor package)."@en ;
                     rdfs:label "originating facility"@en .


###  http://fdri.ceh.ac.uk/vocab/metadata/originatingProgramme
:originatingProgramme rdf:type owl:ObjectProperty ;
                      rdfs:domain :ObservationDataset ;
                      rdfs:range :EnvironmentalMonitoringProgramme ;
                      rdfs:comment "The environmental monitoring programme that intiated the activities that resulted in the production of this dataset."@en ;
                      rdfs:label "originating programme"@en .


###  http://fdri.ceh.ac.uk/vocab/metadata/originatingSite
:originatingSite rdf:type owl:ObjectProperty ;
                 rdfs:subPropertyOf :originatingFacility ;
                 rdfs:comment "Relates a dataset of observations to the Environmental Monitoring Site from which the observations originated."@en ;
                 rdfs:label "originating site"@en .


###  http://fdri.ceh.ac.uk/vocab/metadata/parameter
:parameter rdf:type owl:ObjectProperty ;
           rdfs:subPropertyOf owl:topObjectProperty ;
           rdfs:range :ConfigurationParameter ;
           rdfs:comment "Relates a Data Processing Method to one of the paramters that the method takes, or a Data Processing Configuration Argument to the parameter that it provides a value for."@en ;
           rdfs:label "parameter"@en .


###  http://fdri.ceh.ac.uk/vocab/metadata/programme
:programme rdf:type owl:ObjectProperty ;
           rdfs:range :EnvironmentalMonitoringProgramme ;
           rdfs:comment "Relates a Programme Catalog to the Environmental Monitoring Programme that the catalog covers."@en ;
           rdfs:label "programme"@en .


###  http://fdri.ceh.ac.uk/vocab/metadata/property
:property rdf:type owl:ObjectProperty ;
          rdfs:range :Variable ;
          rdfs:comment "References the `fdri:Variable` which describes the property for which an `fdri:Annotation` provides a value or value series."@en ;
          rdfs:label "property"@en .


###  http://fdri.ceh.ac.uk/vocab/metadata/qualifier
:qualifier rdf:type owl:ObjectProperty ;
           rdfs:range :Annotation ;
           rdfs:comment "Provides an additional qualifier value for an annotation value."@en ;
           rdfs:label "qualifier"@en .


###  http://fdri.ceh.ac.uk/vocab/metadata/regionScheme
:regionScheme rdf:type owl:ObjectProperty ;
              rdfs:subPropertyOf dcat:themeTaxonomy ;
              rdfs:range :RegionScheme ;
              rdfs:comment "References a controlled list of geographical regions that are referenced by the catalog."@en ;
              rdfs:label "region scheme"@en .


###  http://fdri.ceh.ac.uk/vocab/metadata/status
:status rdf:type owl:ObjectProperty ;
        rdfs:comment "The operational status of an Environmental Monitoring System."@en ;
        rdfs:label "status"@en .


###  http://fdri.ceh.ac.uk/vocab/metadata/uses
:uses rdf:type owl:ObjectProperty ;
      rdfs:range :TimeSeriesDefinition ;
      rdfs:comment "Relates a Time Series Plan for the production of some Time Series to the Time Series Definitions that define the input Time Series used by the plan."@en ;
      rdfs:label "uses"@en .


###  http://fdri.ceh.ac.uk/vocab/metadata/utilises
:utilises rdf:type owl:ObjectProperty ;
          rdfs:domain :EnvironmentalMonitoringProgramme ;
          rdfs:range [ rdf:type owl:Class ;
                       owl:unionOf ( :EnvironmentalMonitoringFacility
                                     :EnvironmentalMonitoringNetwork
                                   )
                     ] ;
          rdfs:label "Relates an Environmental Monitoring Programme to the Environmental Monitoring Facility or Environmental Monitoring Network used by the programme in the delivery of its outputs."@en ,
                     "utilises"@en .


###  http://fdri.ceh.ac.uk/vocab/metadata/valueStatistic
:valueStatistic rdf:type owl:ObjectProperty ;
                rdfs:range :ValueStatistic ;
                rdfs:comment "Relates an aggregated data resource to the type of aggregation applied."@en ;
                rdfs:label "value statistic"@en .


###  http://fdri.ceh.ac.uk/vocab/metadata/valueType
:valueType rdf:type owl:ObjectProperty ;
           rdfs:comment """The type of the value of the enclosing resource.

On a `schema:PropertyValue` resource, the value of this property should be the IRI of the datatype of `minValue`, `maxValue` and/or `value` or the IRI of the class of the resource referenced by `valueReference`.

On an `fdri:Measure` resource, this property specifies the expected datatype for observed values of the `fdri:Measure`."""@en ;
           rdfs:label "value type"@en .


###  http://fdri.ceh.ac.uk/vocab/metadata/variable
:variable rdf:type owl:ObjectProperty ;
          rdfs:range :Variable ;
          rdfs:comment "Relates a Measure to the Variable that is measured."@en ;
          rdfs:label "variable"@en .


###  http://fdri.ceh.ac.uk/vocab/metadata/wasModifiedBy
:wasModifiedBy rdf:type owl:ObjectProperty ;
               rdfs:subPropertyOf prov:wasInfluencedBy ;
               rdfs:domain :ObservationDataset ;
               rdfs:comment "Relates a resource to the activity that modified the resource in some way."@en ;
               rdfs:label "was modified by"@en .


###  http://purl.org/dc/terms/replaces
dct:replaces rdf:type owl:ObjectProperty .


###  http://purl.org/dc/terms/type
dct:type rdf:type owl:ObjectProperty .


###  http://schema.org/unit
schema:unit rdf:type owl:ObjectProperty ;
            rdfs:domain <http://qudt.org/schema/qudt/Unit> .


###  http://schema.org/valueReference
schema:valueReference rdf:type owl:ObjectProperty .


###  http://www.w3.org/2003/01/geo/wgs84_pos#location
geo:location rdf:type owl:ObjectProperty .


###  http://www.w3.org/ns/prov#wasInfluencedBy
prov:wasInfluencedBy rdfs:subPropertyOf ssn:wasOriginatedBy .


###  http://www.w3.org/ns/sosa/hasFeatureOfInterest
sosa:hasFeatureOfInterest schema:domainIncludes :EnvironmentalMonitoringFacility .


###  http://www.w3.org/ns/sosa/observedProperty
sosa:observedProperty schema:domainIncludes :ObservationDataset .


#################################################################
#    Data properties
#################################################################

###  http://fdri.ceh.ac.uk/vocab/metadata/aggregationPeriod
:aggregationPeriod rdf:type owl:DatatypeProperty ;
                   rdfs:range xsd:duration ;
                   rdfs:comment "The duration of time over which an time-series aggregation applies."@en ;
                   rdfs:label "aggregation period"@en .


###  http://fdri.ceh.ac.uk/vocab/metadata/altitude
:altitude rdf:type owl:DatatypeProperty ;
          rdfs:range xsd:decimal ;
          rdfs:comment "Height above sea-level measured in metres."@en ;
          rdfs:label "altitude"@en .


###  http://fdri.ceh.ac.uk/vocab/metadata/assetNumber
:assetNumber rdf:type owl:DatatypeProperty ;
             rdfs:range xsd:string ;
             rdfs:comment "An identifier assigned to a piece of infrastructure or equipment by the entity that is responsible for the management of that item."@en ;
             rdfs:label "asset number"@en .


###  http://fdri.ceh.ac.uk/vocab/metadata/calibrationDue
:calibrationDue rdf:type owl:DatatypeProperty ;
                rdfs:range [ rdf:type rdfs:Datatype ;
                             owl:unionOf ( xsd:date
                                           xsd:dateTime
                                         )
                           ] ;
                rdfs:comment "The date or date/time by which an instrument is due to be (re)calibrated."@en ;
                rdfs:label "calibration due"@en .


###  http://fdri.ceh.ac.uk/vocab/metadata/dateOfDisposal
:dateOfDisposal rdf:type owl:DatatypeProperty ;
                rdfs:subPropertyOf dct:date ;
                rdfs:range xsd:date ;
                rdfs:comment "The date on which an item was disposed of by the entity that manged it up to that date."@en ;
                rdfs:label "date of disposal"@en .


###  http://fdri.ceh.ac.uk/vocab/metadata/dateOfPurchase
:dateOfPurchase rdf:type owl:DatatypeProperty ;
                rdfs:subPropertyOf dct:date ;
                rdfs:range xsd:date ;
                rdfs:comment "The date on which an item was purchased by the entity that manages it."@en ;
                rdfs:label "date of purchase" .


###  http://fdri.ceh.ac.uk/vocab/metadata/dependencyNote
:dependencyNote rdf:type owl:DatatypeProperty ;
                rdfs:subPropertyOf :deploymentNote ;
                rdfs:comment "A note regarding dependency of the enclosing Deployment."@en ;
                rdfs:label "dependency note"@en .


###  http://fdri.ceh.ac.uk/vocab/metadata/deployedDepth
:deployedDepth rdf:type owl:DatatypeProperty ;
               rdfs:range xsd:decimal ;
               rdfs:comment "The depth (in metres) below ground level at which an environmental monitoring system is deployed."@en ;
               rdfs:label "deployed depth"@en .


###  http://fdri.ceh.ac.uk/vocab/metadata/deployedHeight
:deployedHeight rdf:type owl:DatatypeProperty ;
                rdfs:range xsd:decimal ;
                rdfs:comment "The height (in metres) above ground level at which an environmental monitoring system is deployed."@en ;
                rdfs:label "deployed height"@en .


###  http://fdri.ceh.ac.uk/vocab/metadata/deploymentNote
:deploymentNote rdf:type owl:DatatypeProperty ;
                rdfs:subPropertyOf owl:topDataProperty ;
                rdfs:comment """A note provinding some additional contextual information about the deployment of a system. 

More specific sub-properties `fdri:dependencyNote` and `fdri:deploymentVariance` are provided to capture specific types of note and should be used where appropriate in preference to this property."""@en ;
                rdfs:label "deployment note"@en .


###  http://fdri.ceh.ac.uk/vocab/metadata/deploymentPosition
:deploymentPosition rdf:type owl:DatatypeProperty ;
                    rdfs:range rdf:langString ;
                    rdfs:comment "Descriptive information about the positioning of an Environmental Monitoring System as the result of the containing StaticDeployment activity"@en ;
                    rdfs:label "deployment position"@en .


###  http://fdri.ceh.ac.uk/vocab/metadata/deploymentVariance
:deploymentVariance rdf:type owl:DatatypeProperty ;
                    rdfs:subPropertyOf :deploymentNote ;
                    rdfs:range rdf:langString ;
                    rdfs:comment "Descriptive information about the way in which the deployment of an Environmental Monitoring System differs from the standard deployment of a system of its type."@en ;
                    rdfs:label "deployment variance"@en .


###  http://fdri.ceh.ac.uk/vocab/metadata/elevation
:elevation rdf:type owl:DatatypeProperty ;
           rdfs:subPropertyOf owl:topDataProperty ;
           rdfs:range xsd:decimal ;
           rdfs:comment "The height offset of a relative location from its origin, measured in metres."@en ;
           rdfs:label "elevation"@en .


###  http://fdri.ceh.ac.uk/vocab/metadata/isMobile
:isMobile rdf:type owl:DatatypeProperty ;
          rdfs:range xsd:boolean ;
          rdfs:comment "True if this Environmental Monitoring Facility is not static when reporting measurements. e.g. a UAV, ship"@en ;
          rdfs:label "is mobile"@en .


###  http://fdri.ceh.ac.uk/vocab/metadata/offsetEast
:offsetEast rdf:type owl:DatatypeProperty ;
            rdfs:subPropertyOf owl:topDataProperty ;
            rdfs:range xsd:decimal ;
            rdfs:comment "The easterly offset of a relative location from its origin, measured in metres."@en ;
            rdfs:label "offset east"@en .


###  http://fdri.ceh.ac.uk/vocab/metadata/offsetNorth
:offsetNorth rdf:type owl:DatatypeProperty ;
             rdfs:subPropertyOf owl:topDataProperty ;
             rdfs:range xsd:decimal ;
             rdfs:comment "The northerly offset of a relative location from its origin measured in metres."@en ;
             rdfs:label "offset north"@en .


###  http://fdri.ceh.ac.uk/vocab/metadata/periodicity
:periodicity rdf:type owl:DatatypeProperty ;
             rdfs:subPropertyOf owl:topDataProperty ;
             rdfs:range xsd:duration ;
             rdfs:comment "The duration over which an time-based aggregation applies."@en ;
             rdfs:label "periodicity"@en .


###  http://fdri.ceh.ac.uk/vocab/metadata/procedurePeriodicity
:procedurePeriodicity rdf:type owl:DatatypeProperty ;
                      rdfs:range xsd:duration ;
                      rdfs:comment "How frequently a process or procedure should be carried out."@en ;
                      rdfs:label "procedure periodicity"@en .


###  http://fdri.ceh.ac.uk/vocab/metadata/removeData
:removeData rdf:type owl:DatatypeProperty ;
            rdfs:range xsd:boolean ;
            rdfs:comment "True if data that was measured during the existence of a Fault should be removed from the observation dataset."@en ;
            rdfs:label "remove data"@en .


###  http://fdri.ceh.ac.uk/vocab/metadata/repository
:repository rdf:type owl:DatatypeProperty ;
            rdfs:range xsd:anyURI ;
            schema:domainIncludes prov:SoftwareAgent ;
            rdfs:comment "The IRI of the source control repository which holds the source code for a prov:SoftwareAgent."@en ;
            rdfs:label "source control repository"@en .


###  http://fdri.ceh.ac.uk/vocab/metadata/repositoryPath
:repositoryPath rdf:type owl:DatatypeProperty ;
                rdfs:comment "A repository-relative path to the files or directories that contain the data processing configuration values."@en ;
                rdfs:label "source control repository path"@en .


###  http://fdri.ceh.ac.uk/vocab/metadata/resolution
:resolution rdf:type owl:DatatypeProperty ;
            rdfs:subPropertyOf owl:topDataProperty ;
            rdfs:range xsd:duration ;
            rdfs:comment "The duration between the individual measurements that are aggregated to produce an aggregate value."@en ;
            rdfs:label "resolution"@en .


###  http://fdri.ceh.ac.uk/vocab/metadata/serialNumber
:serialNumber rdf:type owl:DatatypeProperty ;
              rdfs:range xsd:string ;
              rdfs:comment "The unique identifier assigned to a piece of equipment by its manufacturer."@en ;
              rdfs:label "serial number"@en .


###  http://fdri.ceh.ac.uk/vocab/metadata/siteVariance
:siteVariance rdf:type owl:DatatypeProperty ;
              rdfs:range rdf:langString ;
              rdfs:comment "Descriptive information about the way in which the layout of an Environmental Monitoring Facility differs from the standard layout for a facility of its type."@en ;
              rdfs:label "site variance"@en .


###  http://fdri.ceh.ac.uk/vocab/metadata/sourceBucket
:sourceBucket rdf:type owl:DatatypeProperty ;
              rdfs:range xsd:string ;
              rdfs:comment "A reference to the AWS S3 bucket that contains the data for an FDRI dataset."@en ;
              rdfs:label "source bucket"@en .


###  http://fdri.ceh.ac.uk/vocab/metadata/sourceColumnName
:sourceColumnName rdf:type owl:DatatypeProperty ;
                  rdfs:range xsd:string ;
                  rdfs:comment "The name of the column within a source dataset that contain values for an FDRI dataset."@en ;
                  rdfs:label "source column name"@en .


###  http://fdri.ceh.ac.uk/vocab/metadata/sourceDataset
:sourceDataset rdf:type owl:DatatypeProperty ;
               rdfs:range xsd:string ;
               rdfs:comment "The name of the dataset in an AWS S3 bucket which contains the values for an FDRI dataset."@en ;
               rdfs:label "source dataset"@en .


###  http://fdri.ceh.ac.uk/vocab/metadata/storageLocation
:storageLocation rdf:type owl:DatatypeProperty ;
                 rdfs:range xsd:string ;
                 rdfs:comment "The place in which a piece of infrastructure is currently stored."@en ;
                 rdfs:label "storage location"@en .


###  http://fdri.ceh.ac.uk/vocab/metadata/unitName
:unitName rdf:type owl:DatatypeProperty ;
          rdfs:domain :Variable ;
          rdfs:range rdf:langString ;
          rdfs:comment "Provides the display label to use for the unit of measurement of a Complex Observable Property."@en ;
          rdfs:label "unit name"@en .


###  http://www.w3.org/2002/07/owl#topDataProperty
owl:topDataProperty rdfs:domain :Deployment .


###  http://www.w3.org/2003/01/geo/wgs84_pos#lat
geo:lat rdf:type owl:DatatypeProperty ;
        rdfs:domain geo:SpatialThing ;
        rdfs:comment "The WGS84 latitude of a SpatialThing (decimal degrees)." ;
        rdfs:label "latitude" .


###  http://www.w3.org/2003/01/geo/wgs84_pos#long
geo:long rdf:type owl:DatatypeProperty ;
         rdfs:domain geo:SpatialThing ;
         rdfs:comment "The WGS84 longitude of a SpatialThing (decimal degrees)." ;
         rdfs:label "longitude" .


#################################################################
#    Classes
#################################################################

###  http://fdri.ceh.ac.uk/vocab/metadata/ActivityType
:ActivityType rdf:type owl:Class ;
              rdfs:subClassOf skos:Concept ,
                              [ rdf:type owl:Restriction ;
                                owl:onProperty skos:inScheme ;
                                owl:allValuesFrom :ActivityTypeScheme
                              ] ;
              rdfs:comment "A Concept which defines a category of activity."@en ;
              rdfs:label "Activity Type"@en .


###  http://fdri.ceh.ac.uk/vocab/metadata/ActivityTypeScheme
:ActivityTypeScheme rdf:type owl:Class ;
                    rdfs:subClassOf skos:ConceptScheme ;
                    rdfs:comment "A concept scheme that manages a controlled list of activity types."@en ;
                    rdfs:label "Activity Type Scheme"@en .


###  http://fdri.ceh.ac.uk/vocab/metadata/Agent
:Agent rdf:type owl:Class ;
       rdfs:subClassOf dcat:Resource ,
                       prov:Agent ;
       rdfs:comment "An Agent is something that has responsibility for an activity that takes place, for the existence or modification of some resource, or for the activity of another Agent."@en ;
       rdfs:label "Agent"@en .


###  http://fdri.ceh.ac.uk/vocab/metadata/Aggregation
:Aggregation rdf:type owl:Class ;
             rdfs:subClassOf skos:Concept ,
                             [ rdf:type owl:Restriction ;
                               owl:onProperty :valueStatistic ;
                               owl:cardinality "1"^^xsd:nonNegativeInteger
                             ] ,
                             [ rdf:type owl:Restriction ;
                               owl:onProperty :periodicity ;
                               owl:cardinality "1"^^xsd:nonNegativeInteger
                             ] ,
                             [ rdf:type owl:Restriction ;
                               owl:onProperty :resolution ;
                               owl:maxCardinality "1"^^xsd:nonNegativeInteger
                             ] ;
             rdfs:comment "Represents the aggregation of all values collected with a given frequency (fdri:resolution) over a given period of time (fdri:periodicity) using a given aggregation method (fdri:valueStatistic)."@en ;
             rdfs:label "Aggregation"@en .


###  http://fdri.ceh.ac.uk/vocab/metadata/Annotation
:Annotation rdf:type owl:Class ;
            rdfs:subClassOf [ rdf:type owl:Restriction ;
                              owl:onProperty :hasValue ;
                              owl:minCardinality "0"^^xsd:nonNegativeInteger
                            ] ,
                            [ rdf:type owl:Restriction ;
                              owl:onProperty :hasValueSeries ;
                              owl:minCardinality "0"^^xsd:nonNegativeInteger
                            ] ,
                            [ rdf:type owl:Restriction ;
                              owl:onProperty :property ;
                              owl:cardinality "1"^^xsd:nonNegativeInteger
                            ] ;
            rdfs:comment """Annotations provide an extension point to the FDRI metadata model to allow a more diverse range of metadata to be captured than is explicitly allowed for in the model.

Each Annotation instance provides either a single value (`fdri:hasValue`) or a time-based series of values (`fdri:hasValueSeries`) for a single property (`fdri:property`)."""@en ;
            rdfs:label "Annotation"@en .


###  http://fdri.ceh.ac.uk/vocab/metadata/CatchmentScheme
:CatchmentScheme rdf:type owl:Class ;
                 rdfs:subClassOf skos:ConceptScheme ;
                 rdfs:comment "A concept scheme consisting of Catchment concepts."@en ;
                 rdfs:label "Catchment Scheme"@en .


###  http://fdri.ceh.ac.uk/vocab/metadata/ConfigurationArgument
:ConfigurationArgument rdf:type owl:Class ;
                       rdfs:subClassOf [ rdf:type owl:Restriction ;
                                         owl:onProperty :hasValue ;
                                         owl:cardinality "1"^^xsd:nonNegativeInteger
                                       ] ,
                                       [ rdf:type owl:Restriction ;
                                         owl:onProperty :parameter ;
                                         owl:cardinality "1"^^xsd:nonNegativeInteger
                                       ] ;
                       rdfs:comment "Represents a single argument passed to a configuration method as part of an `fdri:ConfigurationItem`."@en ;
                       rdfs:label "Data Processing Configuration Argument"@en .


###  http://fdri.ceh.ac.uk/vocab/metadata/ConfigurationItem
:ConfigurationItem rdf:type owl:Class ;
                   rdfs:subClassOf [ rdf:type owl:Restriction ;
                                     owl:onProperty dct:replaces ;
                                     owl:allValuesFrom :ConfigurationItem
                                   ] ,
                                   [ rdf:type owl:Restriction ;
                                     owl:onProperty :argument ;
                                     owl:minCardinality "0"^^xsd:nonNegativeInteger
                                   ] ,
                                   [ rdf:type owl:Restriction ;
                                     owl:onProperty :method ;
                                     owl:minCardinality "1"^^xsd:nonNegativeInteger
                                   ] ,
                                   [ rdf:type owl:Restriction ;
                                     owl:onProperty :observationInterval ;
                                     owl:minCardinality "0"^^xsd:nonNegativeInteger
                                   ] ,
                                   [ rdf:type owl:Restriction ;
                                     owl:onProperty :interval ;
                                     owl:cardinality "1"^^xsd:nonNegativeInteger
                                   ] ;
                   rdfs:comment """Represents the configuration of a single data processing method to be applied to a subset of observations as part of a data processing pipeline run.

The property `fdri:method` references the concept that defines the data processing method applied. Each argument passed to the data processing method is provided through an `fdri:argument` property.

The property `fdri:interval` indicates the period of time during which this configuration item is/was used. The property `fdri:observationInterval` indicates the date range of the measurements that the configuration item applies to."""@en ;
                   rdfs:label "Data Processing Configuration Item"@en .


###  http://fdri.ceh.ac.uk/vocab/metadata/ConfigurationParameter
:ConfigurationParameter rdf:type owl:Class ;
                        rdfs:subClassOf skos:Concept ,
                                        [ rdf:type owl:Restriction ;
                                          owl:onProperty skos:inScheme ;
                                          owl:allValuesFrom :ConfigurationParameterScheme
                                        ] ;
                        rdfs:comment "Represents a single parameter that may be passed to an `fdri:DataProcessingMethod` as part of a data processing pipeline."@en ;
                        rdfs:label "Configuration Parameter"@en .


###  http://fdri.ceh.ac.uk/vocab/metadata/ConfigurationParameterScheme
:ConfigurationParameterScheme rdf:type owl:Class ;
                              rdfs:subClassOf skos:ConceptScheme ;
                              rdfs:comment "A concept scheme that manages a controlled list of configuration parameters."@en ;
                              rdfs:label "Configuration Parameter Scheme"@en .


###  http://fdri.ceh.ac.uk/vocab/metadata/ConfigurationProperty
:ConfigurationProperty rdf:type owl:Class ;
                       rdfs:subClassOf skos:Concept ,
                                       [ rdf:type owl:Restriction ;
                                         owl:onProperty skos:inScheme ;
                                         owl:allValuesFrom :ConfigurationPropertyScheme
                                       ] ;
                       rdfs:comment """A property of a system or process which may be altered in order to affect the way in which that system or process behaves.

Instances of this class are used to define the properties by which the behaviour of `fdri:EnvironmentalMonitoringSystem`s may be constrained or modified."""@en ;
                       rdfs:label "Configuration Property"@en .


###  http://fdri.ceh.ac.uk/vocab/metadata/ConfigurationPropertyScheme
:ConfigurationPropertyScheme rdf:type owl:Class ;
                             rdfs:subClassOf skos:ConceptScheme ;
                             rdfs:comment "A Concept Scheme that manages a collection of configuration property concepts."@en ;
                             rdfs:label "Configuration Property Scheme"@en .


###  http://fdri.ceh.ac.uk/vocab/metadata/ConfigurationValueSeries
:ConfigurationValueSeries rdf:type owl:Class ;
                          rdfs:subClassOf :PropertyValueSeries ,
                                          [ rdf:type owl:Restriction ;
                                            owl:onProperty dct:type ;
                                            owl:allValuesFrom :ConfigurationProperty
                                          ] ;
                          rdfs:comment "A resources which provides the current and historically configured values for some configuration property."@en ;
                          rdfs:label "Configuration Value Series"@en .


###  http://fdri.ceh.ac.uk/vocab/metadata/DataProcessingConfiguration
:DataProcessingConfiguration rdf:type owl:Class ;
                             rdfs:subClassOf dcat:Resource ,
                                             prov:Plan ,
                                             [ rdf:type owl:Restriction ;
                                               owl:onProperty :appliesToFacility ;
                                               owl:minCardinality "0"^^xsd:nonNegativeInteger
                                             ] ,
                                             [ rdf:type owl:Restriction ;
                                               owl:onProperty :appliesToTimeSeries ;
                                               owl:minCardinality "0"^^xsd:nonNegativeInteger
                                             ] ,
                                             [ rdf:type owl:Restriction ;
                                               owl:onProperty :appliesToVariable ;
                                               owl:minCardinality "0"^^xsd:nonNegativeInteger
                                             ] ,
                                             [ rdf:type owl:Restriction ;
                                               owl:onProperty dct:type ;
                                               owl:minQualifiedCardinality "0"^^xsd:nonNegativeInteger ;
                                               owl:onClass :DataProcessingConfigurationType
                                             ] ;
                             rdfs:comment """The configuration information which is used by a data processing activity to control the way in which the processing activity behaves.

A Data Processing Configuration is defined as a sub-type of `prov:Plan` allowing it to be associated with an Actitvity via the `prov:qualifiedAssociation` property."""@en ;
                             rdfs:label "Data Processing Configuration"@en .


###  http://fdri.ceh.ac.uk/vocab/metadata/DataProcessingConfigurationType
:DataProcessingConfigurationType rdf:type owl:Class ;
                                 rdfs:subClassOf skos:Concept ,
                                                 [ rdf:type owl:Restriction ;
                                                   owl:onProperty skos:inScheme ;
                                                   owl:allValuesFrom :DataProcessingConfigurationTypeScheme
                                                 ] ;
                                 rdfs:comment "A Concept which defines a category of data processing configuration."@en ;
                                 rdfs:label "Data Processing Configuration Type"@en .


###  http://fdri.ceh.ac.uk/vocab/metadata/DataProcessingConfigurationTypeScheme
:DataProcessingConfigurationTypeScheme rdf:type owl:Class ;
                                       rdfs:subClassOf skos:ConceptScheme ;
                                       rdfs:comment "A Concept Scheme which manages a controlled list of Data Processing Configuration Type concepts."@en ;
                                       rdfs:label "Data Processing Configuration Type Scheme"@en .


###  http://fdri.ceh.ac.uk/vocab/metadata/DataProcessingMethod
:DataProcessingMethod rdf:type owl:Class ;
                      rdfs:subClassOf skos:Concept ,
                                      [ rdf:type owl:Restriction ;
                                        owl:onProperty :parameter ;
                                        owl:minQualifiedCardinality "0"^^xsd:nonNegativeInteger ;
                                        owl:onClass :ConfigurationParameter
                                      ] ;
                      rdfs:comment "A Concept which represents a data processing methodology/procedure and the parameters it can take."@en ;
                      rdfs:label "Data Processing Method"@en .


###  http://fdri.ceh.ac.uk/vocab/metadata/Deployment
:Deployment rdf:type owl:Class ;
            rdfs:subClassOf prov:Activity ,
                            ssn:Deployment ,
                            [ rdf:type owl:Restriction ;
                              owl:onProperty ssn:deployedOnPlatform ;
                              owl:allValuesFrom :EnvironmentalMonitoringPlatform
                            ] ,
                            [ rdf:type owl:Restriction ;
                              owl:onProperty ssn:deployedSystem ;
                              owl:allValuesFrom :EnvironmentalMonitoringSystem
                            ] ,
                            [ rdf:type owl:Restriction ;
                              owl:onProperty :dependencyNote ;
                              owl:minCardinality "0"^^xsd:nonNegativeInteger
                            ] ,
                            [ rdf:type owl:Restriction ;
                              owl:onProperty :deploymentNote ;
                              owl:minCardinality "0"^^xsd:nonNegativeInteger
                            ] ,
                            [ rdf:type owl:Restriction ;
                              owl:onProperty :deploymentVariance ;
                              owl:minCardinality "0"^^xsd:nonNegativeInteger
                            ] ;
            rdfs:comment """Describes the deployment of one or more systems of sensors for some purpose.

A deployment may be associated with a platform on which the sensors or systems were deployed."""@en ;
            rdfs:label "Deployment"@en .


###  http://fdri.ceh.ac.uk/vocab/metadata/EnvironmentalDomain
:EnvironmentalDomain rdf:type owl:Class ;
                     rdfs:subClassOf skos:Concept ,
                                     [ rdf:type owl:Restriction ;
                                       owl:onProperty skos:inScheme ;
                                       owl:allValuesFrom :EnvironmentalDomainScheme
                                     ] ;
                     rdfs:comment "A broad aspect of study of the natural environment."@en ;
                     rdfs:label "Environmental Domain"@en .


###  http://fdri.ceh.ac.uk/vocab/metadata/EnvironmentalDomainScheme
:EnvironmentalDomainScheme rdf:type owl:Class ;
                           rdfs:subClassOf skos:ConceptScheme ;
                           rdfs:comment "A controlled vocabulary of Environmental Domain concepts."@en ;
                           rdfs:label "Environmental Domain Scheme"@en .


###  http://fdri.ceh.ac.uk/vocab/metadata/EnvironmentalMonitoringFacility
:EnvironmentalMonitoringFacility rdf:type owl:Class ;
                                 rdfs:subClassOf dcat:Resource ,
                                                 [ rdf:type owl:Restriction ;
                                                   owl:onProperty :environmentalDomain ;
                                                   owl:allValuesFrom skos:Concept
                                                 ] ,
                                                 [ rdf:type owl:Restriction ;
                                                   owl:onProperty dct:type ;
                                                   owl:allValuesFrom :EnvironmentalMonitoringFacilityType
                                                 ] ,
                                                 [ rdf:type owl:Restriction ;
                                                   owl:onProperty prov:qualifiedAttribution ;
                                                   owl:allValuesFrom :RelatedPartyAttribution
                                                 ] ,
                                                 [ rdf:type owl:Restriction ;
                                                   owl:onProperty sosa:hasFeatureOfInterest ;
                                                   owl:allValuesFrom :GeospatialFeatureOfInterest
                                                 ] ,
                                                 [ rdf:type owl:Restriction ;
                                                   owl:onProperty sosa:observes ;
                                                   owl:allValuesFrom sosa:ObservableProperty
                                                 ] ,
                                                 [ rdf:type owl:Restriction ;
                                                   owl:onProperty :measures ;
                                                   owl:minCardinality "0"^^xsd:nonNegativeInteger
                                                 ] ,
                                                 [ rdf:type owl:Restriction ;
                                                   owl:onProperty :wasModifiedBy ;
                                                   owl:minCardinality "0"^^xsd:nonNegativeInteger
                                                 ] ,
                                                 [ rdf:type owl:Restriction ;
                                                   owl:onProperty prov:qualifiedAttribution ;
                                                   owl:minCardinality "0"^^xsd:nonNegativeInteger
                                                 ] ,
                                                 [ rdf:type owl:Restriction ;
                                                   owl:onProperty prov:wasGeneratedBy ;
                                                   owl:minCardinality "0"^^xsd:nonNegativeInteger
                                                 ] ,
                                                 [ rdf:type owl:Restriction ;
                                                   owl:onProperty prov:wasInvalidatedBy ;
                                                   owl:minCardinality "0"^^xsd:nonNegativeInteger
                                                 ] ,
                                                 [ rdf:type owl:Restriction ;
                                                   owl:onProperty :operatingPeriod ;
                                                   owl:maxCardinality "1"^^xsd:nonNegativeInteger
                                                 ] ,
                                                 [ rdf:type owl:Restriction ;
                                                   owl:onProperty dct:type ;
                                                   owl:maxCardinality "1"^^xsd:nonNegativeInteger
                                                 ] ,
                                                 [ rdf:type owl:Restriction ;
                                                   owl:onProperty geos:hasBoundingBox ;
                                                   owl:maxCardinality "1"^^xsd:nonNegativeInteger
                                                 ] ,
                                                 [ rdf:type owl:Restriction ;
                                                   owl:onProperty geos:hasCentroid ;
                                                   owl:maxCardinality "1"^^xsd:nonNegativeInteger
                                                 ] ,
                                                 [ rdf:type owl:Restriction ;
                                                   owl:onProperty geos:hasGeometry ;
                                                   owl:maxCardinality "1"^^xsd:nonNegativeInteger
                                                 ] ,
                                                 [ rdf:type owl:Restriction ;
                                                   owl:onProperty sosa:hasFeatureOfInterest ;
                                                   owl:maxCardinality "1"^^xsd:nonNegativeInteger
                                                 ] ,
                                                 [ rdf:type owl:Restriction ;
                                                   owl:onProperty spatialrelations:easting ;
                                                   owl:maxQualifiedCardinality "1"^^xsd:nonNegativeInteger ;
                                                   owl:onDataRange xsd:string
                                                 ] ,
                                                 [ rdf:type owl:Restriction ;
                                                   owl:onProperty spatialrelations:northing ;
                                                   owl:maxQualifiedCardinality "1"^^xsd:nonNegativeInteger ;
                                                   owl:onDataRange xsd:string
                                                 ] ,
                                                 [ rdf:type owl:Restriction ;
                                                   owl:onProperty :isMobile ;
                                                   owl:maxCardinality "1"^^xsd:nonNegativeInteger
                                                 ] ,
                                                 [ rdf:type owl:Restriction ;
                                                   owl:onProperty geo:lat ;
                                                   owl:maxQualifiedCardinality "1"^^xsd:nonNegativeInteger ;
                                                   owl:onDataRange xsd:string
                                                 ] ,
                                                 [ rdf:type owl:Restriction ;
                                                   owl:onProperty geo:long ;
                                                   owl:maxQualifiedCardinality "1"^^xsd:nonNegativeInteger ;
                                                   owl:onDataRange xsd:string
                                                 ] ;
                                 rdfs:comment """A piece of infrastructure used by an environmental monitoring programme for some purpose.

The derived classes `fdri:EnvironmentalMonitoringSite`, `fdri:EnvironmentalMonitoringPlatform`,  `fdri:EnvironmentalMonitoringSystem`, and `fdri:EnvironmentalMonitoringSensor` should be used in preference to this class."""@en ;
                                 rdfs:label "Environmental Monitoring Facility"@en .


###  http://fdri.ceh.ac.uk/vocab/metadata/EnvironmentalMonitoringFacilityType
:EnvironmentalMonitoringFacilityType rdf:type owl:Class ;
                                     rdfs:subClassOf skos:Concept ,
                                                     [ rdf:type owl:Restriction ;
                                                       owl:onProperty skos:inScheme ;
                                                       owl:allValuesFrom :EnvironmentalMonitoringFacilityTypeScheme
                                                     ] ,
                                                     [ rdf:type owl:Restriction ;
                                                       owl:onProperty prov:qualifiedAssociation ;
                                                       owl:allValuesFrom :RelatedPartyAttribution
                                                     ] ,
                                                     [ rdf:type owl:Restriction ;
                                                       owl:onProperty :measures ;
                                                       owl:minCardinality "0"^^xsd:nonNegativeInteger
                                                     ] ;
                                     rdfs:comment "A Concept that represents a class of Environmental Monitoring Facility as defined by the monitoring programme that uses it."@en ;
                                     rdfs:label "Environmental Monitoring Facility Type"@en .


###  http://fdri.ceh.ac.uk/vocab/metadata/EnvironmentalMonitoringFacilityTypeScheme
:EnvironmentalMonitoringFacilityTypeScheme rdf:type owl:Class ;
                                           rdfs:subClassOf skos:ConceptScheme ;
                                           rdfs:comment "A controlled vocabulary of monitoring facility types."@en ;
                                           rdfs:label "Environmental Monitoring Facility Type Scheme"@en .


###  http://fdri.ceh.ac.uk/vocab/metadata/EnvironmentalMonitoringNetwork
:EnvironmentalMonitoringNetwork rdf:type owl:Class ;
                                rdfs:subClassOf [ rdf:type owl:Restriction ;
                                                  owl:onProperty :contains ;
                                                  owl:allValuesFrom :EnvironmentalMonitoringFacility
                                                ] ;
                                rdfs:comment "A collection of infrastructure elements (`fdri:EnvironmentalMonitoringFacility`) which are used together for some environmental monitoring purpose."@en ;
                                rdfs:label "Environmental Monitoring Network"@en .


###  http://fdri.ceh.ac.uk/vocab/metadata/EnvironmentalMonitoringPlatform
:EnvironmentalMonitoringPlatform rdf:type owl:Class ;
                                 rdfs:subClassOf :EnvironmentalMonitoringFacility ,
                                                 sosa:Platform ;
                                 rdfs:comment """A piece of infrastructure at a site that is used in the monitoring of the environment at that site.

An Environmental Monitoring Platform may be a physical piece of infrastructure such as a post in the ground, a raised platform or a hole in the ground. It may also be used to represent a \"slot\" in the site infrastructure to which sensors may be serially deployed over time in order to monitor the same phenomenon.

An Environmental Monitoring Platform may host (`sosa:hosts`) any number of systems (`fdri:EnvironmentalMonitoringSystem`). It may also be the target of a Deployment (`fdri:deployedOnPlatform` on `fdri:Deployment`) of some `fdri:EnvironmentalMonitoringSystem`. This latter formulation is preferred when the system(s) deployed on the platform may change over time."""@en ;
                                 rdfs:label "Environmental Monitoring Platform"@en .


###  http://fdri.ceh.ac.uk/vocab/metadata/EnvironmentalMonitoringProgramme
:EnvironmentalMonitoringProgramme rdf:type owl:Class ;
                                  rdfs:subClassOf [ rdf:type owl:Restriction ;
                                                    owl:onProperty :utilises ;
                                                    owl:minCardinality "0"^^xsd:nonNegativeInteger
                                                  ] ;
                                  rdfs:comment """An activity which undertakes the monitoring of some aspect(s) of the natural environment.

An Environmental Monitoring Programme may make use of (`fdri:utilises`) any number of Environmental Monitoring Networks (`fdri:EnvironmentalMonitoringNetwork`) and/or Environmental Monitoring Facilities (`fdri:EnvironmentalMonitoringFacility`) in order to achieive its goals."""@en ;
                                  rdfs:label "Environmental Monitoring Programme"@en .


###  http://fdri.ceh.ac.uk/vocab/metadata/EnvironmentalMonitoringSensor
:EnvironmentalMonitoringSensor rdf:type owl:Class ;
                               rdfs:subClassOf :EnvironmentalMonitoringSystem ,
                                               sosa:Sensor ,
                                               [ rdf:type owl:Restriction ;
                                                 owl:onProperty :certification ;
                                                 owl:maxCardinality "1"^^xsd:nonNegativeInteger
                                               ] ,
                                               [ rdf:type owl:Restriction ;
                                                 owl:onProperty :status ;
                                                 owl:maxQualifiedCardinality "1"^^xsd:nonNegativeInteger ;
                                                 owl:onClass :SystemStatus
                                               ] ,
                                               [ rdf:type owl:Restriction ;
                                                 owl:onProperty :assetNumber ;
                                                 owl:maxCardinality "1"^^xsd:nonNegativeInteger
                                               ] ,
                                               [ rdf:type owl:Restriction ;
                                                 owl:onProperty :dateOfDisposal ;
                                                 owl:maxCardinality "1"^^xsd:nonNegativeInteger
                                               ] ,
                                               [ rdf:type owl:Restriction ;
                                                 owl:onProperty :dateOfPurchase ;
                                                 owl:maxCardinality "1"^^xsd:nonNegativeInteger
                                               ] ,
                                               [ rdf:type owl:Restriction ;
                                                 owl:onProperty :storageLocation ;
                                                 owl:maxCardinality "1"^^xsd:nonNegativeInteger
                                               ] ;
                               rdfs:comment "A device which responds to a stimulus such as a change in the environment and reports a resulting observation."@en ;
                               rdfs:label "Environmental Monitoring Sensor"@en .


###  http://fdri.ceh.ac.uk/vocab/metadata/EnvironmentalMonitoringSite
:EnvironmentalMonitoringSite rdf:type owl:Class ;
                             rdfs:subClassOf :EnvironmentalMonitoringFacility ,
                                             sosa:Platform ,
                                             [ rdf:type owl:Restriction ;
                                               owl:onProperty sosa:hosts ;
                                               owl:allValuesFrom sosa:Platform
                                             ] ,
                                             [ rdf:type owl:Restriction ;
                                               owl:onProperty :siteVariance ;
                                               owl:minCardinality "0"^^xsd:nonNegativeInteger
                                             ] ,
                                             [ rdf:type owl:Restriction ;
                                               owl:onProperty :altitude ;
                                               owl:maxCardinality "1"^^xsd:nonNegativeInteger
                                             ] ;
                             rdfs:comment """A geo-spatial location which contains infrastructure elements to which environmental monitoring systms are deployed.

An Environmental Monitoring Site may host any number of systems (`fdri:EnvironmentalMonitoringSystem`) and it may be the target of any number of deployments (`fdri:deployedOnPlatform` on `fdri:Deployment`) of systems. This latter formulation should be used when the system(s) deployed to a site may change over time. 

If information is available regarding the platforms (`fdri:EnvironmentalMonitoringPlatform`) at a site, then hosting and deployment relationships should target the platform(s) rather than the site where possible."""@en ;
                             rdfs:label "Environmental Monitoring Site"@en .


###  http://fdri.ceh.ac.uk/vocab/metadata/EnvironmentalMonitoringSystem
:EnvironmentalMonitoringSystem rdf:type owl:Class ;
                               rdfs:subClassOf :EnvironmentalMonitoringFacility ,
                                               ssn:System ,
                                               [ rdf:type owl:Restriction ;
                                                 owl:onProperty :configuration ;
                                                 owl:allValuesFrom :ConfigurationValueSeries
                                               ] ,
                                               [ rdf:type owl:Restriction ;
                                                 owl:onProperty dct:type ;
                                                 owl:allValuesFrom :EnvironmentalMonitoringFacilityType
                                               ] ,
                                               [ rdf:type owl:Restriction ;
                                                 owl:onProperty ssn:hasSubSystem ;
                                                 owl:allValuesFrom :EnvironmentalMonitoringSystem
                                               ] ,
                                               [ rdf:type owl:Restriction ;
                                                 owl:onProperty :calibrationDue ;
                                                 owl:maxCardinality "1"^^xsd:nonNegativeInteger
                                               ] ,
                                               [ rdf:type owl:Restriction ;
                                                 owl:onProperty :serialNumber ;
                                                 owl:maxCardinality "1"^^xsd:nonNegativeInteger
                                               ] ;
                               rdfs:comment "An abstraction for a pieces of environmental monitoring infrastructure that may be deployed to provide observations of environmental features of interest."@en ;
                               rdfs:label "Environmental Monitoring System"@en .


###  http://fdri.ceh.ac.uk/vocab/metadata/EnvironmentalMonitoringSystemType
:EnvironmentalMonitoringSystemType rdf:type owl:Class ;
                                   rdfs:subClassOf :EnvironmentalMonitoringFacilityType ,
                                                   [ rdf:type owl:Restriction ;
                                                     owl:onProperty :hasProcedure ;
                                                     owl:allValuesFrom :Procedure
                                                   ] ,
                                                   [ rdf:type owl:Restriction ;
                                                     owl:onProperty :hasProcedure ;
                                                     owl:minCardinality "0"^^xsd:nonNegativeInteger
                                                   ] ,
                                                   [ rdf:type owl:Restriction ;
                                                     owl:onProperty dcat:keyword ;
                                                     owl:minCardinality "0"^^xsd:nonNegativeInteger
                                                   ] ;
                                   rdfs:comment """A concept that defines a classification of monitoring system type.

System type classification includes both broad functional classification (e.g. anenometer), and more narrow make and model classification."""@en ;
                                   rdfs:label "Environmental Monitoring System Type"@en .


###  http://fdri.ceh.ac.uk/vocab/metadata/ExternalDataProcessingConfiguration
:ExternalDataProcessingConfiguration rdf:type owl:Class ;
                                     rdfs:subClassOf :DataProcessingConfiguration ,
                                                     [ rdf:type owl:Restriction ;
                                                       owl:onProperty :repository ;
                                                       owl:cardinality "1"^^xsd:nonNegativeInteger
                                                     ] ,
                                                     [ rdf:type owl:Restriction ;
                                                       owl:onProperty :repositoryPath ;
                                                       owl:maxCardinality "1"^^xsd:nonNegativeInteger
                                                     ] ,
                                                     [ rdf:type owl:Restriction ;
                                                       owl:onProperty dcat:version ;
                                                       owl:maxQualifiedCardinality "1"^^xsd:nonNegativeInteger ;
                                                       owl:onDataRange xsd:string
                                                     ] ;
                                     rdfs:comment """A Data Processing Configuration whose values are maintained in a system external to the FDRI metadata store.

The `dct:version` property of this class SHOULD be used to provide the commit hash, tag or other stable identifier of a specifiic version of the referenced configuration data in the source repository.

The `dct:type` property of this class SHOULD be used to reference the `fdri:DataProcessingConfigurationType` concept that defines the category of configuration data provided by the configuration."""@en ;
                                     rdfs:label "External Data Processing Configuration"@en .


###  http://fdri.ceh.ac.uk/vocab/metadata/FacilityGroup
:FacilityGroup rdf:type owl:Class ;
               rdfs:subClassOf dcat:Resource ,
                               [ rdf:type owl:Restriction ;
                                 owl:onProperty dct:type ;
                                 owl:allValuesFrom :FacilityGroupType
                               ] ,
                               [ rdf:type owl:Restriction ;
                                 owl:onProperty :hasMember ;
                                 owl:minQualifiedCardinality "0"^^xsd:nonNegativeInteger ;
                                 owl:onClass :EnvironmentalMonitoringFacility
                               ] ,
                               [ rdf:type owl:Restriction ;
                                 owl:onProperty :hasRepresentativePoint ;
                                 owl:minCardinality "0"^^xsd:nonNegativeInteger
                               ] ,
                               [ rdf:type owl:Restriction ;
                                 owl:onProperty geos:hasBoundingBox ;
                                 owl:minCardinality "0"^^xsd:nonNegativeInteger
                               ] ,
                               [ rdf:type owl:Restriction ;
                                 owl:onProperty geos:hasCentroid ;
                                 owl:minCardinality "0"^^xsd:nonNegativeInteger
                               ] ,
                               [ rdf:type owl:Restriction ;
                                 owl:onProperty geos:hasGeometry ;
                                 owl:minCardinality "0"^^xsd:nonNegativeInteger
                               ] ,
                               [ rdf:type owl:Restriction ;
                                 owl:onProperty dct:type ;
                                 owl:maxCardinality "1"^^xsd:nonNegativeInteger
                               ] ,
                               [ rdf:type owl:Restriction ;
                                 owl:onProperty spatialrelations:easting ;
                                 owl:maxQualifiedCardinality "1"^^xsd:nonNegativeInteger ;
                                 owl:onDataRange xsd:string
                               ] ,
                               [ rdf:type owl:Restriction ;
                                 owl:onProperty spatialrelations:northing ;
                                 owl:maxQualifiedCardinality "1"^^xsd:nonNegativeInteger ;
                                 owl:onDataRange xsd:string
                               ] ,
                               [ rdf:type owl:Restriction ;
                                 owl:onProperty geo:lat ;
                                 owl:maxQualifiedCardinality "1"^^xsd:nonNegativeInteger ;
                                 owl:onDataRange xsd:string
                               ] ,
                               [ rdf:type owl:Restriction ;
                                 owl:onProperty geo:long ;
                                 owl:maxQualifiedCardinality "1"^^xsd:nonNegativeInteger ;
                                 owl:onDataRange xsd:string
                               ] ;
               rdfs:comment """Represents a collection of related Environmental Monitoring Facilities.

Facility Groups may be geographic (e.g. region, catchment), administrative (e.g. local authority, commisioning group) or created for any other purpose.

Membership may be expressed directly using the `fdri:hasMember` property, or indirectly (with an optional temporal constraint) by creating `fdri:FacilityGroupMembership` instances."""@en ;
               rdfs:label "Environmental Monitoring Facility Group"@en .


###  http://fdri.ceh.ac.uk/vocab/metadata/FacilityGroupMembership
:FacilityGroupMembership rdf:type owl:Class ;
                         rdfs:subClassOf [ rdf:type owl:Restriction ;
                                           owl:onProperty :group ;
                                           owl:cardinality "1"^^xsd:nonNegativeInteger
                                         ] ,
                                         [ rdf:type owl:Restriction ;
                                           owl:onProperty :interval ;
                                           owl:cardinality "1"^^xsd:nonNegativeInteger
                                         ] ,
                                         [ rdf:type owl:Restriction ;
                                           owl:onProperty :member ;
                                           owl:cardinality "1"^^xsd:nonNegativeInteger
                                         ] ;
                         rdfs:comment "Represents an optionally time-bounded membership of an `fdri:FacilityGroup` by some `fdri:EnvironmenalMonitoringFacility`."@en ;
                         rdfs:label "Facility Group Membership"@en .


###  http://fdri.ceh.ac.uk/vocab/metadata/FacilityGroupType
:FacilityGroupType rdf:type owl:Class ;
                   rdfs:subClassOf skos:Concept ,
                                   [ rdf:type owl:Restriction ;
                                     owl:onProperty skos:inScheme ;
                                     owl:allValuesFrom :FacilityGroupTypeScheme
                                   ] ;
                   rdfs:comment "A concept representing the nature of a facility group. e.g. catchment, region, project."@en ;
                   rdfs:label "Facility Group Type"@en .


###  http://fdri.ceh.ac.uk/vocab/metadata/FacilityGroupTypeScheme
:FacilityGroupTypeScheme rdf:type owl:Class ;
                         rdfs:subClassOf skos:ConceptScheme ;
                         rdfs:comment "A controlled vocabulary of monitoring facility group types."@en ;
                         rdfs:label "Environmental Monitoring Facility Group Type Scheme"@en .


###  http://fdri.ceh.ac.uk/vocab/metadata/Fault
:Fault rdf:type owl:Class ;
       rdfs:subClassOf [ rdf:type owl:Restriction ;
                         owl:onProperty :affectedFacility ;
                         owl:someValuesFrom owl:Thing
                       ] ,
                       [ rdf:type owl:Restriction ;
                         owl:onProperty :affectedVariable ;
                         owl:someValuesFrom :Variable
                       ] ,
                       [ rdf:type owl:Restriction ;
                         owl:onProperty :interval ;
                         owl:qualifiedCardinality "1"^^xsd:nonNegativeInteger ;
                         owl:onClass dct:PeriodOfTime
                       ] ,
                       [ rdf:type owl:Restriction ;
                         owl:onProperty :removeData ;
                         owl:maxCardinality "1"^^xsd:nonNegativeInteger
                       ] ;
       rdfs:comment """A record of a fault that affects the capture of one or more variables (`fdri:affectedVariable`) by one or more monitoring facilities (`fdri:affectedFacility`) for a given period of time (`fdri:interval).

A fault may or may not require that data collected for the affected variables by the affected facilities be removed from the published datasets (`fdri:removeData`). 

A persistent or unresolved fault may be represented by using an interval with no defined end time."""@en ;
       rdfs:label "Fault"@en .


###  http://fdri.ceh.ac.uk/vocab/metadata/GeospatialFeatureOfInterest
:GeospatialFeatureOfInterest rdf:type owl:Class ;
                             rdfs:subClassOf sosa:Sample ,
                                             [ rdf:type owl:Restriction ;
                                               owl:onProperty geos:hasGeometry ;
                                               owl:allValuesFrom geos:Geometry
                                             ] ,
                                             [ rdf:type owl:Restriction ;
                                               owl:onProperty geos:hasGeometry ;
                                               owl:minCardinality "1"^^xsd:nonNegativeInteger
                                             ] ,
                                             [ rdf:type owl:Restriction ;
                                               owl:onProperty :hasRepresentativePoint ;
                                               owl:cardinality "1"^^xsd:nonNegativeInteger
                                             ] ,
                                             [ rdf:type owl:Restriction ;
                                               owl:onProperty spatialrelations:easting ;
                                               owl:maxQualifiedCardinality "1"^^xsd:nonNegativeInteger ;
                                               owl:onDataRange xsd:string
                                             ] ,
                                             [ rdf:type owl:Restriction ;
                                               owl:onProperty spatialrelations:northing ;
                                               owl:maxQualifiedCardinality "1"^^xsd:nonNegativeInteger ;
                                               owl:onDataRange xsd:string
                                             ] ,
                                             [ rdf:type owl:Restriction ;
                                               owl:onProperty geo:lat ;
                                               owl:maxQualifiedCardinality "1"^^xsd:nonNegativeInteger ;
                                               owl:onDataRange xsd:string
                                             ] ,
                                             [ rdf:type owl:Restriction ;
                                               owl:onProperty geo:long ;
                                               owl:maxQualifiedCardinality "1"^^xsd:nonNegativeInteger ;
                                               owl:onDataRange xsd:string
                                             ] ;
                             rdfs:comment "A Feature of Interest with a geospatial location."@en ;
                             rdfs:label "Geo-spatial Feature Of Interest"@en .


###  http://fdri.ceh.ac.uk/vocab/metadata/InternalDataProcessingConfiguration
:InternalDataProcessingConfiguration rdf:type owl:Class ;
                                     rdfs:subClassOf :DataProcessingConfiguration ,
                                                     [ rdf:type owl:Restriction ;
                                                       owl:onProperty :hadConfigurationItem ;
                                                       owl:minCardinality "0"^^xsd:nonNegativeInteger
                                                     ] ,
                                                     [ rdf:type owl:Restriction ;
                                                       owl:onProperty :hasCurrentConfigurationItem ;
                                                       owl:minCardinality "0"^^xsd:nonNegativeInteger
                                                     ] ;
                                     rdfs:comment """A data processing configuration whose values are stored in the FDRI metadata service.

Configuration values are conveyed by a collection of Configiration Items (`fdri:ConfigurationItem`) referenced from this item using the properties `fdri:hasCurrentConfiguration` for items which represent currently active values, and `fdri:hadConfiguration` for items which represent historically active values.

A current configuration MAY consist of multiple `fdri:ConfigurationItem` instances providing configuration details for different data processing methods."""@en ;
                                     rdfs:label "Internal Data Processing Configuration"@en .


###  http://fdri.ceh.ac.uk/vocab/metadata/Measure
:Measure rdf:type owl:Class ;
         rdfs:subClassOf skos:Concept ,
                         [ rdf:type owl:Restriction ;
                           owl:onProperty skos:inScheme ;
                           owl:allValuesFrom :MeasureScheme
                         ] ,
                         [ rdf:type owl:Restriction ;
                           owl:onProperty :hasUnit ;
                           owl:cardinality "1"^^xsd:nonNegativeInteger
                         ] ,
                         [ rdf:type owl:Restriction ;
                           owl:onProperty :variable ;
                           owl:cardinality "1"^^xsd:nonNegativeInteger
                         ] ,
                         [ rdf:type owl:Restriction ;
                           owl:onProperty :aggregation ;
                           owl:maxCardinality "1"^^xsd:nonNegativeInteger
                         ] ,
                         [ rdf:type owl:Restriction ;
                           owl:onProperty :valueType ;
                           owl:maxCardinality "1"^^xsd:nonNegativeInteger
                         ] ;
         rdfs:comment "Represents the measurement of a variable (fdri:variable) as recorded in a dataset using some consistent measurement unit (fdri:hasUnit) and an optional aggregation (fdri:aggregation)." ;
         rdfs:label "Measure"@en .


###  http://fdri.ceh.ac.uk/vocab/metadata/MeasureScheme
:MeasureScheme rdf:type owl:Class ;
               rdfs:subClassOf skos:ConceptScheme ;
               rdfs:comment "A controlled vocabulary of variable measures."@en ;
               rdfs:label "Measure Scheme"@en .


###  http://fdri.ceh.ac.uk/vocab/metadata/ObservationDataset
:ObservationDataset rdf:type owl:Class ;
                    rdfs:subClassOf dcat:Dataset ,
                                    [ rdf:type owl:Restriction ;
                                      owl:onProperty dcat:inSeries ;
                                      owl:allValuesFrom :ObservationDatasetSeries
                                    ] ,
                                    [ rdf:type owl:Restriction ;
                                      owl:onProperty :measure ;
                                      owl:minCardinality "0"^^xsd:nonNegativeInteger
                                    ] ,
                                    [ rdf:type owl:Restriction ;
                                      owl:onProperty :originatingFacility ;
                                      owl:minCardinality "0"^^xsd:nonNegativeInteger
                                    ] ,
                                    [ rdf:type owl:Restriction ;
                                      owl:onProperty :originatingProgramme ;
                                      owl:minCardinality "0"^^xsd:nonNegativeInteger
                                    ] ,
                                    [ rdf:type owl:Restriction ;
                                      owl:onProperty :originatingSite ;
                                      owl:minCardinality "0"^^xsd:nonNegativeInteger
                                    ] ,
                                    [ rdf:type owl:Restriction ;
                                      owl:onProperty :wasModifiedBy ;
                                      owl:minCardinality "0"^^xsd:nonNegativeInteger
                                    ] ,
                                    [ rdf:type owl:Restriction ;
                                      owl:onProperty sosa:hasFeatureOfInterest ;
                                      owl:minCardinality "0"^^xsd:nonNegativeInteger
                                    ] ,
                                    [ rdf:type owl:Restriction ;
                                      owl:onProperty sosa:observedProperty ;
                                      owl:minQualifiedCardinality "0"^^xsd:nonNegativeInteger ;
                                      owl:onClass :Variable
                                    ] ;
                    rdfs:comment """A dataset that provides values for Measures from some Environmental Monitoring Facility or Programme.

The property `fdri:measure` should be use to specify the Measures recorded by the dataset and `sosa:observedProperty` should be used to specify the Variables measured by those measures.

It is recommended that every dataset should specify the feature(s) of interest (sosa:hasFeatureOfInterest) observed by the measures in the dataset, and the originating programme (fdri:originatingProgramme) for the data. Datasets that provide observations from static sites should also reference these using the `fdri:originatingSite` property."""@en ;
                    rdfs:label "Observation Dataset"@en .


###  http://fdri.ceh.ac.uk/vocab/metadata/ObservationDatasetSeries
:ObservationDatasetSeries rdf:type owl:Class ;
                          rdfs:subClassOf :ObservationDataset ,
                                          dcat:DatasetSeries ;
                          rdfs:comment "A Dataset Series that groups a collection of related Observation Datasets together."@en ;
                          rdfs:label "Observation Dataset Series"@en .


###  http://fdri.ceh.ac.uk/vocab/metadata/Organization
:Organization rdf:type owl:Class ;
              rdfs:subClassOf :Agent ;
              rdfs:comment "A social or legal institution such as a company, society etc."@en ;
              rdfs:label "Organization"@en .


###  http://fdri.ceh.ac.uk/vocab/metadata/Person
:Person rdf:type owl:Class ;
        rdfs:subClassOf :Agent ;
        rdfs:comment "A natural person."@en ;
        rdfs:label "Person"@en .


###  http://fdri.ceh.ac.uk/vocab/metadata/Procedure
:Procedure rdf:type owl:Class ;
           rdfs:subClassOf dcat:Resource ,
                           prov:Plan ,
                           [ rdf:type owl:Restriction ;
                             owl:onProperty dct:type ;
                             owl:allValuesFrom :ProcedureType
                           ] ,
                           [ rdf:type owl:Restriction ;
                             owl:onProperty :procedurePeriodicity ;
                             owl:maxCardinality "1"^^xsd:nonNegativeInteger
                           ] ;
           rdfs:comment """A process follwed by an Agent (`fdri:Agent`) during the execution of an Activity (`prov:Activity`).

The categorization of the procedure SHOULD be indicated using the `dct:type` property referencing an `fdri:ProcedureType` concept.

The periodicity (`fdri:procedurePeriodicity`) property SHOULD be used to capture the expected frequency of execution of the Procedure."""@en ;
           rdfs:label "Procedure"@en .


###  http://fdri.ceh.ac.uk/vocab/metadata/ProcedureType
:ProcedureType rdf:type owl:Class ;
               rdfs:subClassOf skos:Concept ,
                               [ rdf:type owl:Restriction ;
                                 owl:onProperty skos:inScheme ;
                                 owl:allValuesFrom :ProcedureTypeScheme
                               ] ;
               rdfs:comment "A concept which defines a category or type of `fdri:Procedure`."@en ;
               rdfs:label "Procedure Type"@en .


###  http://fdri.ceh.ac.uk/vocab/metadata/ProcedureTypeScheme
:ProcedureTypeScheme rdf:type owl:Class ;
                     rdfs:subClassOf skos:ConceptScheme ;
                     rdfs:comment "A controlled vocabulary of types or categories of procedure that might be undertaken by an Agent as (part of) an Activity."@en ;
                     rdfs:label "Procedure Type Scheme"@en .


###  http://fdri.ceh.ac.uk/vocab/metadata/ProcessingLevel
:ProcessingLevel rdf:type owl:Class ;
                 rdfs:subClassOf skos:Concept ,
                                 [ rdf:type owl:Restriction ;
                                   owl:onProperty skos:inScheme ;
                                   owl:allValuesFrom :ProcessingLevelScheme
                                 ] ;
                 rdfs:comment "A concept which defines a level of data processing that has been applied to a dataset."@en ;
                 rdfs:label "Processing Level"@en .


###  http://fdri.ceh.ac.uk/vocab/metadata/ProcessingLevelScheme
:ProcessingLevelScheme rdf:type owl:Class ;
                       rdfs:subClassOf skos:ConceptScheme ;
                       rdfs:comment "A controlled vocabulary of the levels of data processing which may be applied to a dataaset."@en ;
                       rdfs:label "Processing Level Scheme"@en .


###  http://fdri.ceh.ac.uk/vocab/metadata/ProgrammeCatalog
:ProgrammeCatalog rdf:type owl:Class ;
                  rdfs:subClassOf dcat:Catalog ,
                                  [ rdf:type owl:Restriction ;
                                    owl:onProperty :programme ;
                                    owl:cardinality "1"^^xsd:nonNegativeInteger
                                  ] .


###  http://fdri.ceh.ac.uk/vocab/metadata/PropertyValue
:PropertyValue rdf:type owl:Class ;
               rdfs:subClassOf schema:PropertyValue ,
                               [ rdf:type owl:Restriction ;
                                 owl:onProperty :qualifier ;
                                 owl:minCardinality "0"^^xsd:nonNegativeInteger
                               ] ;
               rdfs:comment "A structured representation of the value of a property, allowing for values that are simple values, value ranges, or classifications."@en ;
               rdfs:label "Property Value"@en .


###  http://fdri.ceh.ac.uk/vocab/metadata/PropertyValueSeries
:PropertyValueSeries rdf:type owl:Class ;
                     rdfs:subClassOf [ rdf:type owl:Restriction ;
                                       owl:onProperty :hadValue ;
                                       owl:minCardinality "0"^^xsd:nonNegativeInteger
                                     ] ,
                                     [ rdf:type owl:Restriction ;
                                       owl:onProperty :hasCurrentValue ;
                                       owl:maxCardinality "1"^^xsd:nonNegativeInteger
                                     ] ;
                     rdfs:comment "An record of values of a property. The currently active/valid value is given by `fdri:hasCurrentValue` and historic values are given by `fdri:hadValue`."@en ;
                     rdfs:label "Property Value Series"@en .


###  http://fdri.ceh.ac.uk/vocab/metadata/QualityObservation
:QualityObservation rdf:type owl:Class ;
                    rdfs:subClassOf sosa:Observation ,
                                    [ rdf:type owl:Restriction ;
                                      owl:onProperty sosa:hasFeatureOfInterest ;
                                      owl:allValuesFrom dcat:Dataset
                                    ] ;
                    rdfs:comment "A type of `sosa:Observation` that provides quality metrics for some `dcat:Dataset`"@en ;
                    rdfs:label "Quality Observation"@en .


###  http://fdri.ceh.ac.uk/vocab/metadata/RegionScheme
:RegionScheme rdf:type owl:Class ;
              rdfs:subClassOf skos:ConceptScheme ;
              rdfs:comment "A controlled vocabulary of Regions."@en ;
              rdfs:label "Region Scheme"@en .


###  http://fdri.ceh.ac.uk/vocab/metadata/RelatedPartyAttribution
:RelatedPartyAttribution rdf:type owl:Class ;
                         rdfs:subClassOf prov:Attribution ,
                                         [ rdf:type owl:Restriction ;
                                           owl:onProperty prov:agent ;
                                           owl:allValuesFrom :Agent
                                         ] ,
                                         [ rdf:type owl:Restriction ;
                                           owl:onProperty prov:hadRole ;
                                           owl:allValuesFrom :RelatedPartyRole
                                         ] ;
                         rdfs:comment "An association between an Agent and the role that they play in relation to the referencing resource."@en ;
                         rdfs:label "Related Party Attribution"@en .


###  http://fdri.ceh.ac.uk/vocab/metadata/RelatedPartyRole
:RelatedPartyRole rdf:type owl:Class ;
                  rdfs:subClassOf skos:Concept ,
                                  [ rdf:type owl:Restriction ;
                                    owl:onProperty skos:inScheme ;
                                    owl:allValuesFrom :RelatedPartyRoleScheme
                                  ] ;
                  rdfs:comment "A concept that defines the role an `fdri:Agent` may play in relation to some resource."@en ;
                  rdfs:label "Related Party Role"@en .


###  http://fdri.ceh.ac.uk/vocab/metadata/RelatedPartyRoleScheme
:RelatedPartyRoleScheme rdf:type owl:Class ;
                        rdfs:subClassOf skos:ConceptScheme ;
                        rdfs:comment "A concept scheme that defines a controlled vocabulary for the roles that an Agent may play in relation to other resources."@en ;
                        rdfs:label "Related Party Role Scheme"@en .


###  http://fdri.ceh.ac.uk/vocab/metadata/RelativeLocation
:RelativeLocation rdf:type owl:Class ;
                  rdfs:subClassOf [ rdf:type owl:Restriction ;
                                    owl:onProperty :elevation ;
                                    owl:maxCardinality "1"^^xsd:nonNegativeInteger
                                  ] ,
                                  [ rdf:type owl:Restriction ;
                                    owl:onProperty :offsetEast ;
                                    owl:maxCardinality "1"^^xsd:nonNegativeInteger
                                  ] ,
                                  [ rdf:type owl:Restriction ;
                                    owl:onProperty :offsetNorth ;
                                    owl:maxCardinality "1"^^xsd:nonNegativeInteger
                                  ] ;
                  rdfs:comment "Specifies a geographic point as an offset from some contextually-defined reference point."@en ;
                  rdfs:label "Relative Location"@en .


###  http://fdri.ceh.ac.uk/vocab/metadata/SoftwareAgent
:SoftwareAgent rdf:type owl:Class ;
               rdfs:subClassOf :Agent ,
                               [ rdf:type owl:Restriction ;
                                 owl:onProperty :repositoryPath ;
                                 owl:minCardinality "0"^^xsd:nonNegativeInteger
                               ] ,
                               [ rdf:type owl:Restriction ;
                                 owl:onProperty :repository ;
                                 owl:maxCardinality "1"^^xsd:nonNegativeInteger
                               ] ;
               rdfs:comment "A software system"@en ;
               rdfs:label "Software Agent"@en .


###  http://fdri.ceh.ac.uk/vocab/metadata/SoilType
:SoilType rdf:type owl:Class ;
          rdfs:subClassOf skos:Concept ,
                          [ rdf:type owl:Restriction ;
                            owl:onProperty skos:inScheme ;
                            owl:allValuesFrom :SoilTypeScheme
                          ] ;
          rdfs:comment "A concept that defines a soil type classification."@en ;
          rdfs:label "Soil Type"@en .


###  http://fdri.ceh.ac.uk/vocab/metadata/SoilTypeScheme
:SoilTypeScheme rdf:type owl:Class ;
                rdfs:subClassOf skos:ConceptScheme ;
                rdfs:comment "A concept scheme that defines a controlled vocabulary of soil type classifications."@en ;
                rdfs:label "Soil Type Scheme"@en .


###  http://fdri.ceh.ac.uk/vocab/metadata/StaticDeployment
:StaticDeployment rdf:type owl:Class ;
                  rdfs:subClassOf :Deployment ,
                                  [ rdf:type owl:Restriction ;
                                    owl:onProperty prov:atLocation ;
                                    owl:maxQualifiedCardinality "1"^^xsd:nonNegativeInteger ;
                                    owl:onClass [ rdf:type owl:Class ;
                                                  owl:unionOf ( :RelativeLocation
                                                                geos:Feature
                                                              )
                                                ]
                                  ] ,
                                  [ rdf:type owl:Restriction ;
                                    owl:onProperty :deploymentPosition ;
                                    owl:minCardinality "0"^^xsd:nonNegativeInteger
                                  ] ,
                                  [ rdf:type owl:Restriction ;
                                    owl:onProperty :deployedDepth ;
                                    owl:maxCardinality "1"^^xsd:nonNegativeInteger
                                  ] ,
                                  [ rdf:type owl:Restriction ;
                                    owl:onProperty :deployedHeight ;
                                    owl:maxCardinality "1"^^xsd:nonNegativeInteger
                                  ] ;
                  rdfs:comment "A deployment of a sensor or system of sensors in a fixed relationship to some location."@en ;
                  rdfs:label "Static Deploment"@en .


###  http://fdri.ceh.ac.uk/vocab/metadata/SystemStatus
:SystemStatus rdf:type owl:Class ;
              rdfs:subClassOf skos:Concept ,
                              [ rdf:type owl:Restriction ;
                                owl:onProperty skos:inScheme ;
                                owl:allValuesFrom :SystemStatusScheme
                              ] ;
              rdfs:comment "A concept that defines an operational status category for an Environmental Monitoring System."@en ;
              rdfs:label "System Status"@en .


###  http://fdri.ceh.ac.uk/vocab/metadata/SystemStatusScheme
:SystemStatusScheme rdf:type owl:Class ;
                    rdfs:subClassOf skos:ConceptScheme ;
                    rdfs:comment "A controlled vocabulary of system status categories."@en ;
                    rdfs:label "System Status Scheme"@en .


###  http://fdri.ceh.ac.uk/vocab/metadata/TimeBoundPropertyValue
:TimeBoundPropertyValue rdf:type owl:Class ;
                        rdfs:subClassOf :PropertyValue ,
                                        [ rdf:type owl:Restriction ;
                                          owl:onProperty dct:replaces ;
                                          owl:allValuesFrom :TimeBoundPropertyValue
                                        ] ,
                                        [ rdf:type owl:Restriction ;
                                          owl:onProperty :interval ;
                                          owl:minCardinality "1"^^xsd:nonNegativeInteger
                                        ] ;
                        rdfs:comment "A value with an associated period of time during which the value is/was vaild."@en ;
                        rdfs:label "Time-bound Property Value"@en .


###  http://fdri.ceh.ac.uk/vocab/metadata/TimeSeriesDataset
:TimeSeriesDataset rdf:type owl:Class ;
                   rdfs:subClassOf :ObservationDataset ,
                                   [ rdf:type owl:Restriction ;
                                     owl:onProperty dct:type ;
                                     owl:allValuesFrom :TimeSeriesDefinition
                                   ] ,
                                   [ rdf:type owl:Restriction ;
                                     owl:onProperty :sourceBucket ;
                                     owl:maxCardinality "1"^^xsd:nonNegativeInteger
                                   ] ,
                                   [ rdf:type owl:Restriction ;
                                     owl:onProperty :sourceColumnName ;
                                     owl:maxCardinality "1"^^xsd:nonNegativeInteger
                                   ] ,
                                   [ rdf:type owl:Restriction ;
                                     owl:onProperty :sourceDataset ;
                                     owl:maxCardinality "1"^^xsd:nonNegativeInteger
                                   ] ;
                   rdfs:comment """A Observation Dataset consisting of a collection of values of one or more Measures of some Feature of Interest at regular intervals over a period of time.

This class extends `fdri:ObservationDataset` with metadata properties that assist in the processing of the data through the FDRI data pipeline. `fdri:sourceBucket`, `fdri:sourceDataset` and `fdri:sourceColumnName` are used to access the dataset values. The `dct:type` property references the `fdri:TimeSeriesDefinition` instance which provides processing configuration information for the dataset."""@en ;
                   rdfs:label "Time-Series Dataset"@en .


###  http://fdri.ceh.ac.uk/vocab/metadata/TimeSeriesDefinition
:TimeSeriesDefinition rdf:type owl:Class ;
                      rdfs:subClassOf skos:Concept ,
                                      [ rdf:type owl:Restriction ;
                                        owl:onProperty sosa:observedProperty ;
                                        owl:minCardinality "1"^^xsd:nonNegativeInteger
                                      ] ,
                                      [ rdf:type owl:Restriction ;
                                        owl:onProperty :methodology ;
                                        owl:maxQualifiedCardinality "1"^^xsd:nonNegativeInteger ;
                                        owl:onClass :TimeSeriesPlan
                                      ] ,
                                      [ rdf:type owl:Restriction ;
                                        owl:onProperty :valueStatistic ;
                                        owl:maxCardinality "1"^^xsd:nonNegativeInteger
                                      ] ;
                      rdfs:comment """A representation of a time series of some observed or derived measurement of a variable.

A Time-Series Definition captures the information that is common across multiple Time-Series Datasets that measure or derive values for the same Variable using the same procedure."""@en ;
                      rdfs:label "Time-Series Definition"@en .


###  http://fdri.ceh.ac.uk/vocab/metadata/TimeSeriesPlan
:TimeSeriesPlan rdf:type owl:Class ;
                rdfs:subClassOf :Procedure ,
                                [ rdf:type owl:Restriction ;
                                  owl:onProperty :configuration ;
                                  owl:allValuesFrom :DataProcessingConfiguration
                                ] ,
                                [ rdf:type owl:Restriction ;
                                  owl:onProperty :uses ;
                                  owl:minCardinality "0"^^xsd:nonNegativeInteger
                                ] ;
                rdfs:comment "A procedure which results in the creation or update of instances of a Time-Series Definition (`fdri:TimeSeriesDefinition`) through the application of one or more data processing configurations (`fdri:DataProcessingConfiguration`) to it's input time series."@en ;
                rdfs:label "Time-series Plan"@en .


###  http://fdri.ceh.ac.uk/vocab/metadata/Unit
:Unit rdf:type owl:Class ;
      rdfs:subClassOf skos:Concept ,
                      [ rdf:type owl:Restriction ;
                        owl:onProperty skos:inScheme ;
                        owl:allValuesFrom :UnitScheme
                      ] ;
      rdfs:comment "A Concept which represents a unit of measure of an observable property."@en ;
      rdfs:label "Unit of Measure"@en .


###  http://fdri.ceh.ac.uk/vocab/metadata/UnitScheme
:UnitScheme rdf:type owl:Class ;
            rdfs:subClassOf skos:ConceptScheme ;
            rdfs:comment "A concept scheme providing a controlled vocabulary of units of measure."@en ;
            rdfs:label "Unit of Measure Scheme"@en .


###  http://fdri.ceh.ac.uk/vocab/metadata/ValueStatistic
:ValueStatistic rdf:type owl:Class ;
                rdfs:subClassOf skos:Concept ;
                rdfs:comment "A concept that defines a statistical method for the derivation of a single aggregated value from a series of source values."@en ;
                rdfs:label "Value Statistic"@en .


###  http://fdri.ceh.ac.uk/vocab/metadata/Variable
:Variable rdf:type owl:Class ;
          rdfs:subClassOf skos:Concept ,
                          sosa:ObservableProperty ,
                          iop:Variable ,
                          [ rdf:type owl:Restriction ;
                            owl:onProperty skos:inScheme ;
                            owl:allValuesFrom :VariableScheme
                          ] ;
          rdfs:comment "A variable whose definition also captures additional information about the context of each measurement of the property."@en ;
          rdfs:label "Variable"@en .


###  http://fdri.ceh.ac.uk/vocab/metadata/VariableScheme
:VariableScheme rdf:type owl:Class ;
                rdfs:subClassOf skos:ConceptScheme ;
                rdfs:comment "A concept scheme which manages a controlled set of Variable definitions."@en ;
                rdfs:label "Variable Scheme"@en .


###  http://qudt.org/schema/qudt/Unit
<http://qudt.org/schema/qudt/Unit> rdf:type owl:Class .


###  http://schema.org/PropertyValue
schema:PropertyValue rdf:type owl:Class ;
                     rdfs:subClassOf [ rdf:type owl:Restriction ;
                                       owl:onProperty :valueType ;
                                       owl:maxCardinality "1"^^xsd:nonNegativeInteger
                                     ] ,
                                     [ rdf:type owl:Restriction ;
                                       owl:onProperty schema:unit ;
                                       owl:maxCardinality "1"^^xsd:nonNegativeInteger
                                     ] ,
                                     [ rdf:type owl:Restriction ;
                                       owl:onProperty schema:valueReference ;
                                       owl:maxCardinality "1"^^xsd:nonNegativeInteger
                                     ] .


###  http://www.w3.org/2003/01/geo/wgs84_pos#Point
geo:Point rdf:type owl:Class ;
          rdfs:subClassOf geo:SpatialThing ;
          rdfs:comment """ 
Uniquely identified by lat/long/alt. i.e.

spaciallyIntersects(P1, P2) :- lat(P1, LAT), long(P1, LONG), alt(P1, ALT),
  lat(P2, LAT), long(P2, LONG), alt(P2, ALT).

sameThing(P1, P2) :- type(P1, Point), type(P2, Point), spaciallyIntersects(P1, P2).
  """ ,
                       """A point, typically described using a coordinate system relative to Earth, such as WGS84.
  """ ;
          rdfs:label "point" .


###  http://www.w3.org/2003/01/geo/wgs84_pos#SpatialThing
geo:SpatialThing rdf:type owl:Class ;
                 rdfs:comment """Anything with spatial extent, i.e. size, shape, or position.
 e.g. people, places, bowling balls, as well as abstract areas like cubes.
""" ;
                 rdfs:label "SpatialThing" .


###  http://www.w3.org/ns/dcat#Resource
dcat:Resource rdfs:subClassOf [ rdf:type owl:Restriction ;
                                owl:onProperty :hasAnnotation ;
                                owl:minCardinality "0"^^xsd:nonNegativeInteger
                              ] .


###  http://www.w3.org/ns/prov#Activity
prov:Activity rdfs:subClassOf [ rdf:type owl:Restriction ;
                                owl:onProperty dct:type ;
                                owl:allValuesFrom :ActivityType
                              ] .


###  https://w3id.org/iadopt/ont/Entity
iop:Entity rdf:type owl:Class ;
           rdfs:subClassOf skos:Concept .


###  https://w3id.org/iadopt/ont/Property
iop:Property rdf:type owl:Class ;
             rdfs:subClassOf skos:Concept ;
             rdfs:comment "A type of a characteristic of an `iop:ObjectOfInterest`."@en ;
             rdfs:label "Property"@en .


###  https://w3id.org/iadopt/ont/Variable
iop:Variable rdf:type owl:Class .


#################################################################
#    Annotations
#################################################################

geo: <http://purl.org/dc/elements/1.1/date> "$Date: 2009/04/20 15:00:30 $" ;
     <http://purl.org/dc/elements/1.1/description> """A vocabulary for representing latitude, longitude and 
 altitude information in the WGS84 geodetic reference datum. 
 Version $Id: wgs84_pos.rdf,v 1.22 2009/04/20 15:00:30 timbl Exp $. See http://www.w3.org/2003/01/geo/ for more details.""" ;
     <http://purl.org/dc/elements/1.1/title> "WGS84 Geo Positioning: an RDF vocabulary" ;
     rdfs:comment """
Recent changes to this namespace:
$Log: wgs84_pos.rdf,v $
Revision 1.22  2009/04/20 15:00:30  timbl
Remove the time bits which have been deal with elsewhere eg in iCal.

Revision 1.21  2009/04/20 12:52:47  timbl
try again

Revision 1.20  2009/04/20 12:42:11  timbl
Add Event (edited ages ago and never checked in), and location (following discussion http://chatlogs.planetrdf.com/swig/2009-04-20#T12-36-09)

Revision 1.19  2009/04/20 12:36:31  timbl
Add Event (edited ages ago and never checked in), and location (following discussion http://chatlogs.planetrdf.com/swig/2009-04-20#T12-36-09)

Revision 1.18  2006/02/01 22:01:04  danbri
Clarified that lat and long are decimal degrees, and that alt is decimal metres about local reference ellipsoid

Revision 1.17  2004/02/06 17:38:12  danbri
Fixed a bad commit screwup

Revision 1.15  2003/04/19 11:24:08  danbri
Fixed the typo even more.

Revision 1.14  2003/04/19 11:16:56  danbri
fixed a typo

Revision 1.13  2003/02/19 22:27:27  connolly
relaxed domain constraints on lat/long/alt from Point to SpatialThing

Revision 1.12  2003/01/12 01:41:41  danbri
Trying local copy of XSLT doc.

Revision 1.11  2003/01/12 01:20:18  danbri
added a link to morten's xslt rdfs viewer.

Revision 1.10  2003/01/11 18:56:49  danbri
Removed datatype range from lat and long properties, since they would
have required each occurance of the property to mention the datatype.

Revision 1.9  2003/01/11 11:41:31  danbri
Another typo; repaired rdfs:Property to rdf:Property x4

Revision 1.8  2003/01/11 11:05:02  danbri
Added an rdfs:range for each lat/long/alt property,
http://www.w3.org/2001/XMLSchema#float

Revision 1.7  2003/01/10 20:25:16  danbri
Longer rdfs:comment for Point, trying to be Earth-centric and neutral about
coordinate system(s) at the same time. Feedback welcomed.

Revision 1.6  2003/01/10 20:18:30  danbri
Added CVS log comments into the RDF/XML as an rdfs:comment property of the
vocabulary. Note that this is not common practice (but seems both harmless
and potentially useful).


revision 1.5
date: 2003/01/10 20:14:31;  author: danbri;  state: Exp;  lines: +16 -5
Updated schema:
Added a dc:date, added url for more info. Changed the rdfs:label of the
namespace from gp to geo. Added a class Point, set as the rdfs:domain of
each property. Added XML comment on the lat_long property suggesting that
we might not need it (based on #rdfig commentary from implementors).

revision 1.4
date: 2003/01/10 20:01:07;  author: danbri;  state: Exp;  lines: +6 -5
Fixed typo; several rdfs:about attributes are now rdf:about. Thanks to MortenF in
#rdfig for catching this error.

revision 1.3
date: 2003/01/10 11:59:03;  author: danbri;  state: Exp;  lines: +4 -3
fixed buglet in vocab, added more wgs links

revision 1.2
date: 2003/01/10 11:01:11;  author: danbri;  state: Exp;  lines: +4 -4
Removed alt from the as-a-flat-string property, and switched from
space separated to comma separated.

revision 1.1
date: 2003/01/10 10:53:23;  author: danbri;  state: Exp;
basic geo vocab

""" ;
     rdfs:label "geo" .


geo:lat_long rdfs:comment "A comma-separated representation of a latitude, longitude coordinate." ;
             rdfs:label "lat/long" .


geo:location rdfs:comment """The relation between something and the point, 
 or other geometrical thing in space, where it is.  For example, the realtionship between
 a radio tower and a Point with a given lat and long.
 Or a relationship between a park and its outline as a closed arc of points, or a road and
 its location as a arc (a sequence of points).
 Clearly in practice there will be limit to the accuracy of any such statement, but one would expect
 an accuracy appropriate for the size of the object and uses such as mapping .
 """ ;
             rdfs:label "location" .


sosa:hasUltimateFeatureOfInterest schema:domainIncludes dcat:Dataset .


sosa:isFeatureOfInterestOf schema:rangeIncludes :EnvironmentalMonitoringFacility .


###  Generated by the OWL API (version 4.5.29.2024-05-13T12:11:03Z) https://github.com/owlcs/owlapi
